Weidenbach_Book/IsaSAT_Arena_LLVM.thy
@@ -5,127 +5,32 @@ no_notation WB_More_Refinement.fref ("[_]\<^sub>f _ \<rightarrow> _" [0,60,60] 6
 no_notation WB_More_Refinement.freft ("_ \<rightarrow>\<^sub>f _" [60,60] 60)
 
 
-subsubsection \<open>Code Generation\<close>
-
-
-term arena_el_rel
-
-term xarena_length
-
-definition "arena_el_impl_rel \<equiv> unat_rel' TYPE(32) O arena_el_rel"
-lemmas [fcomp_norm_unfold] = arena_el_impl_rel_def[symmetric]
-
-abbreviation "arena_el_impl_assn \<equiv> pure arena_el_impl_rel"
-
-lemma xarena_length_refine1: "(\<lambda>eli. eli, xarena_length) \<in> [is_Size]\<^sub>f arena_el_rel \<rightarrow> nat_rel"
-  by (auto intro!: frefI simp: arena_el_rel_def split: arena_el.splits)
-
-sepref_definition xarena_len_impl is "RETURN o (\<lambda>eli. eli)" :: "uint32_nat_assn\<^sup>k \<rightarrow>\<^sub>a uint32_nat_assn"
-  by sepref
-  
-lemmas [sepref_fr_rules] = xarena_len_impl.refine[FCOMP xarena_length_refine1]  
-  
-abbreviation "arena_assn \<equiv> al_assn' TYPE(64) arena_el_impl_assn"
-
-
-lemma arena_lifting': 
-  assumes "arena_is_valid_clause_idx a b"
-  shows "Suc 0 \<le> b"
-  and "b < length a"
-  and "is_Size (a ! (b - Suc 0))"
-  using SIZE_SHIFT_def assms
-  by (auto simp: arena_is_valid_clause_idx_def arena_lifting)
 
 (* TODO: Let monadify-phase do this automatically? trade-of: goal-size vs. lost information *) 
 lemma protected_bind_assoc: "Refine_Basic.bind$(Refine_Basic.bind$m$(\<lambda>\<^sub>2x. f x))$(\<lambda>\<^sub>2y. g y) = Refine_Basic.bind$m$(\<lambda>\<^sub>2x. Refine_Basic.bind$(f x)$(\<lambda>\<^sub>2y. g y))" by simp
+
+(* TODO: Move to Bits_Natural in Isabelle-LLVM *)
+lemma nat_and_comm: "a AND b = b AND a" for a b :: nat
+  unfolding bitAND_nat_def by (auto simp: int_and_comm)
+
+lemma AND_upper_nat1: "a AND b \<le> a" for a b :: nat
+proof -
+  have "int a AND int b \<le> int a"
+    by (rule AND_upper1) simp
+  thus ?thesis unfolding bitAND_nat_def by linarith
+qed    
+
+lemma AND_upper_nat2: "a AND b \<le> b" for a b :: nat
+  using AND_upper_nat1[of b a] by (simp add: nat_and_comm)
   
-lemma arena_length_impl_bounds_aux1: 
-  "(ac, a) \<in> unat_rel' TYPE(32) \<Longrightarrow> a < 9223372036854775806"
-  by (auto dest!: in_unat_rel_imp_less_max' simp: max_unat_def)
-
-lemma arena_length_alt: 
-  \<open>arena_length arena i = (
-    let l = xarena_length (arena!(i - snat_const TYPE(64) 1)) 
-    in snat_const TYPE(64) 2 + op_unat_snat_upcast TYPE(64) l)\<close>
-  by (simp add: arena_length_def SIZE_SHIFT_def)  
+lemmas AND_upper_nat1' [simp] = order_trans [OF AND_upper_nat1]
+lemmas AND_upper_nat1'' [simp] = order_le_less_trans [OF AND_upper_nat1]
   
-  
-sepref_definition arena_length_impl 
-  is "uncurry (RETURN oo arena_length)" 
-    :: "[uncurry arena_is_valid_clause_idx]\<^sub>a arena_assn\<^sup>k *\<^sub>a sint64_nat_assn\<^sup>k \<rightarrow> snat_assn' TYPE(64)"
-  unfolding arena_length_alt
-  supply [simp] = max_snat_def max_unat_def arena_length_impl_bounds_aux1
-    and [dest] = arena_lifting'
-  by sepref
+lemmas AND_upper_nat2' [simp] = order_trans [OF AND_upper_nat2]
+lemmas AND_upper_nat2'' [simp] = order_le_less_trans [OF AND_upper_nat2]
   
 
 
-paragraph \<open>Literal at given position\<close>
-
-
-lemma xarena_lit_refine1: "(\<lambda>eli. eli, xarena_lit) \<in> [is_Lit]\<^sub>f arena_el_rel \<rightarrow> nat_lit_rel"
-  by (auto intro!: frefI simp: arena_el_rel_def split: arena_el.splits)
-
-sepref_definition xarena_lit_impl is "RETURN o (\<lambda>eli. eli)" :: "uint32_nat_assn\<^sup>k \<rightarrow>\<^sub>a uint32_nat_assn"
-  by sepref
-
-lemmas [sepref_fr_rules] = xarena_lit_impl.refine[FCOMP xarena_lit_refine1]  
-
-lemma arena_lit_implI:
-  assumes "arena_lit_pre a b"
-  shows "b < length a" "is_Lit (a ! b)"
-  using assms unfolding arena_lit_pre_def arena_is_valid_clause_idx_and_access_def
-  by (fastforce dest: arena_lifting)+
-
-sepref_register arena_lit xarena_lit
-sepref_definition arena_lit_impl 
-  is "uncurry (RETURN oo arena_lit)" 
-    :: "[uncurry arena_lit_pre]\<^sub>a arena_assn\<^sup>k *\<^sub>a sint64_nat_assn\<^sup>k \<rightarrow> unat_lit_assn"
-  supply [intro] = arena_lit_implI
-  unfolding arena_lit_def
-  by sepref
-
-
-      
-paragraph \<open>Status of the clause\<close>
-
-definition "status_impl_rel \<equiv>unat_rel' TYPE(32) O status_rel"
-lemmas [fcomp_norm_unfold] = status_impl_rel_def[symmetric]
-abbreviation "status_impl_assn \<equiv> pure status_impl_rel"
-
-term arena_el_rel
-lemma xarena_status_refine1: "(\<lambda>eli. eli AND 0b11, xarena_status) \<in> [is_Status]\<^sub>f arena_el_rel \<rightarrow> status_rel"
-  by (auto intro!: frefI simp: arena_el_rel_def is_Status_def split: arena_el.split)
-
-sepref_definition xarena_status_impl is "RETURN o (\<lambda>eli. eli AND 0b11)" :: "uint32_nat_assn\<^sup>k \<rightarrow>\<^sub>a uint32_nat_assn"
-  apply (annot_unat_const "TYPE(32)")
-  supply [simp] = max_unat_def
-  by sepref
-
-lemmas [sepref_fr_rules] = xarena_status_impl.refine[FCOMP xarena_status_refine1]  
-
-lemma arena_status_implI:
-  assumes "arena_is_valid_clause_vdom a b"
-  shows "4 \<le> b" "b - 4 < length a" "is_Status (a ! (b-4))"
-  using assms STATUS_SHIFT_def arena_dom_status_iff
-  unfolding arena_is_valid_clause_vdom_def
-  by (auto dest: valid_arena_in_vdom_le_arena)
-
-sepref_register arena_status xarena_status
-sepref_definition arena_status_impl 
-  is "uncurry (RETURN oo arena_status)" 
-    :: "[uncurry arena_is_valid_clause_vdom]\<^sub>a arena_assn\<^sup>k *\<^sub>a sint64_nat_assn\<^sup>k \<rightarrow> status_impl_assn"
-  supply [intro] = arena_status_implI
-  supply [simp] = max_snat_def
-  unfolding arena_status_def STATUS_SHIFT_def
-  apply (annot_snat_const "TYPE(64)")
-  by sepref
-
-
-
-
-
-paragraph \<open>Swap literals\<close>
 
 (* TODO: Move
   TODO: Should be generic algorithm!
@@ -149,22 +54,201 @@ lemma swap_unfold: "swap xs i j = (let
 lemma convert_swap: "WB_More_Refinement_List.swap = IICF_List.swap"
   unfolding WB_More_Refinement_List.swap_def IICF_List.swap_def ..
 
+
+subsubsection \<open>Code Generation\<close>
+
+
+definition "arena_el_impl_rel \<equiv> unat_rel' TYPE(32) O arena_el_rel"
+lemmas [fcomp_norm_unfold] = arena_el_impl_rel_def[symmetric]
+abbreviation "arena_el_impl_assn \<equiv> pure arena_el_impl_rel"
+
+
+paragraph \<open>Arena Element Operations\<close>
+
+context
+  notes [simp] = arena_el_rel_def
+  notes [split] = arena_el.splits
+  notes [intro!] = frefI
+begin  
+
+text \<open>Literal\<close>
+lemma xarena_lit_refine1: "(\<lambda>eli. eli, xarena_lit) \<in> [is_Lit]\<^sub>f arena_el_rel \<rightarrow> nat_lit_rel" by auto
+sepref_definition xarena_lit_impl is "RETURN o (\<lambda>eli. eli)" :: "uint32_nat_assn\<^sup>k \<rightarrow>\<^sub>a uint32_nat_assn" by sepref
+lemmas [sepref_fr_rules] = xarena_lit_impl.refine[FCOMP xarena_lit_refine1]  
+
+lemma ALit_refine1: "(\<lambda>x. x,ALit) \<in> nat_lit_rel \<rightarrow> arena_el_rel" by auto
+sepref_definition ALit_impl is "RETURN o (\<lambda>x. x)" :: "uint32_nat_assn\<^sup>k \<rightarrow>\<^sub>a uint32_nat_assn" by sepref
+lemmas [sepref_fr_rules] = ALit_impl.refine[FCOMP ALit_refine1]  
+
+text \<open>LBD\<close>
+lemma xarena_lbd_refine1: "(\<lambda>eli. eli, xarena_lbd) \<in> [is_LBD]\<^sub>f arena_el_rel \<rightarrow> nat_rel" by auto
+sepref_definition xarena_lbd_impl is "RETURN o (\<lambda>eli. eli)" :: "uint32_nat_assn\<^sup>k \<rightarrow>\<^sub>a uint32_nat_assn" by sepref
+lemmas [sepref_fr_rules] = xarena_lbd_impl.refine[FCOMP xarena_lbd_refine1]
+
+lemma ALBD_refine1: "(\<lambda>eli. eli, ALBD) \<in> nat_rel \<rightarrow> arena_el_rel" by auto
+sepref_definition xarena_ALBD_impl is "RETURN o (\<lambda>eli. eli)" :: "uint32_nat_assn\<^sup>k \<rightarrow>\<^sub>a uint32_nat_assn" by sepref
+lemmas [sepref_fr_rules] = xarena_ALBD_impl.refine[FCOMP ALBD_refine1]
+
+text \<open>Activity\<close>
+lemma xarena_act_refine1: "(\<lambda>eli. eli, xarena_act) \<in> [is_Act]\<^sub>f arena_el_rel \<rightarrow> nat_rel" by auto
+sepref_definition xarena_act_impl is "RETURN o (\<lambda>eli. eli)" :: "uint32_nat_assn\<^sup>k \<rightarrow>\<^sub>a uint32_nat_assn" by sepref
+lemmas [sepref_fr_rules] = xarena_act_impl.refine[FCOMP xarena_act_refine1]  
+
+lemma AAct_refine1: "(\<lambda>x. x,AActivity) \<in> nat_rel \<rightarrow> arena_el_rel" by auto
+sepref_definition AAct_impl is "RETURN o (\<lambda>x. x)" :: "uint32_nat_assn\<^sup>k \<rightarrow>\<^sub>a uint32_nat_assn" by sepref
+lemmas [sepref_fr_rules] = AAct_impl.refine[FCOMP AAct_refine1]  
+
+text \<open>Size\<close>
+lemma xarena_length_refine1: "(\<lambda>eli. eli, xarena_length) \<in> [is_Size]\<^sub>f arena_el_rel \<rightarrow> nat_rel" by auto
+sepref_definition xarena_len_impl is "RETURN o (\<lambda>eli. eli)" :: "uint32_nat_assn\<^sup>k \<rightarrow>\<^sub>a uint32_nat_assn" by sepref
+lemmas [sepref_fr_rules] = xarena_len_impl.refine[FCOMP xarena_length_refine1]  
+
+lemma ASize_refine1: "(\<lambda>x. x,ASize) \<in> nat_rel \<rightarrow> arena_el_rel" by auto
+sepref_definition ASize_impl is "RETURN o (\<lambda>x. x)" :: "uint32_nat_assn\<^sup>k \<rightarrow>\<^sub>a uint32_nat_assn" by sepref
+lemmas [sepref_fr_rules] = ASize_impl.refine[FCOMP ASize_refine1]  
+
+text \<open>Position\<close>
+lemma xarena_pos_refine1: "(\<lambda>eli. eli, xarena_pos) \<in> [is_Pos]\<^sub>f arena_el_rel \<rightarrow> nat_rel" by auto
+sepref_definition xarena_pos_impl is "RETURN o (\<lambda>eli. eli)" :: "uint32_nat_assn\<^sup>k \<rightarrow>\<^sub>a uint32_nat_assn" by sepref
+lemmas [sepref_fr_rules] = xarena_pos_impl.refine[FCOMP xarena_pos_refine1]
+
+lemma APos_refine1: "(\<lambda>x. x,APos) \<in> nat_rel \<rightarrow> arena_el_rel" by auto
+sepref_definition APos_impl is "RETURN o (\<lambda>x. x)" :: "uint32_nat_assn\<^sup>k \<rightarrow>\<^sub>a uint32_nat_assn" by sepref
+lemmas [sepref_fr_rules] = APos_impl.refine[FCOMP APos_refine1]  
+  
+
+text \<open>Status\<close>
+definition "status_impl_rel \<equiv> unat_rel' TYPE(32) O status_rel"
+lemmas [fcomp_norm_unfold] = status_impl_rel_def[symmetric]
+abbreviation "status_impl_assn \<equiv> pure status_impl_rel"
+
+lemma xarena_status_refine1: "(\<lambda>eli. eli AND 0b11, xarena_status) \<in> [is_Status]\<^sub>f arena_el_rel \<rightarrow> status_rel" by (auto simp: is_Status_def)
+sepref_definition xarena_status_impl is "RETURN o (\<lambda>eli. eli AND 0b11)" :: "uint32_nat_assn\<^sup>k \<rightarrow>\<^sub>a uint32_nat_assn"
+  apply (annot_unat_const "TYPE(32)")
+  supply [simp] = max_unat_def
+  by sepref
+lemmas [sepref_fr_rules] = xarena_status_impl.refine[FCOMP xarena_status_refine1]  
+
+lemma xarena_used_refine1: "(\<lambda>eli. eli AND 0b100 \<noteq> 0, xarena_used) \<in> [is_Status]\<^sub>f arena_el_rel \<rightarrow> bool_rel" 
+  by (auto simp: is_Status_def status_rel_def bitfield_rel_def)
+  
+sepref_definition xarena_used_impl is "RETURN o (\<lambda>eli. eli AND 0b100 \<noteq> 0)" :: "uint32_nat_assn\<^sup>k \<rightarrow>\<^sub>a bool1_assn"
+  apply (annot_unat_const "TYPE(32)")
+  supply [simp] = max_unat_def
+  by sepref
+lemmas [sepref_fr_rules] = xarena_used_impl.refine[FCOMP xarena_used_refine1]  
+
+lemma status_eq_refine1: "((=),(=)) \<in> status_rel \<rightarrow> status_rel \<rightarrow> bool_rel"
+  by (auto simp: status_rel_def)
+
+sepref_definition status_eq_impl is "uncurry (RETURN oo (=))" 
+  :: "(unat_assn' TYPE(32))\<^sup>k *\<^sub>a (unat_assn' TYPE(32))\<^sup>k \<rightarrow>\<^sub>a bool1_assn"  
+  by sepref
+
+lemmas [sepref_fr_rules] = status_eq_impl.refine[FCOMP status_eq_refine1]
+
+
+definition "AStatus_impl1 cs used \<equiv> (cs AND unat_const TYPE(32) 0b11) + (if used then unat_const TYPE(32) 0b100 else unat_const TYPE(32) 0b0)"
+lemma AStatus_refine1: "(AStatus_impl1, AStatus) \<in> status_rel \<rightarrow> bool_rel \<rightarrow> arena_el_rel"
+  by (auto simp: status_rel_def bitfield_rel_def AStatus_impl1_def split: if_splits)
+sepref_definition AStatus_impl is "uncurry (RETURN oo AStatus_impl1)" :: "uint32_nat_assn\<^sup>k *\<^sub>a bool1_assn\<^sup>k \<rightarrow>\<^sub>a uint32_nat_assn"
+  unfolding AStatus_impl1_def
+  supply [simp] = max_unat_def and [split] = if_splits
+  by sepref
+lemmas [sepref_fr_rules] = AStatus_impl.refine[FCOMP AStatus_refine1]
+
+
+
+
+
+
+
+subsubsection \<open>Arena Operations\<close>
+
+paragraph \<open>Length\<close>
+
+abbreviation "arena_fast_assn \<equiv> al_assn' TYPE(64) arena_el_impl_assn"
+
+lemma arena_lengthI: 
+  assumes "arena_is_valid_clause_idx a b"
+  shows "Suc 0 \<le> b"
+  and "b < length a"
+  and "is_Size (a ! (b - Suc 0))"
+  using SIZE_SHIFT_def assms
+  by (auto simp: arena_is_valid_clause_idx_def arena_lifting)
+  
+lemma arena_length_impl_bounds_aux1: 
+  "(ac, a) \<in> unat_rel' TYPE(32) \<Longrightarrow> a < 9223372036854775806"
+  by (auto dest!: in_unat_rel_imp_less_max' simp: max_unat_def)
+
+lemma arena_length_alt: 
+  \<open>arena_length arena i = (
+    let l = xarena_length (arena!(i - snat_const TYPE(64) 1)) 
+    in snat_const TYPE(64) 2 + op_unat_snat_upcast TYPE(64) l)\<close>
+  by (simp add: arena_length_def SIZE_SHIFT_def)  
+  
+sepref_register arena_length  
+sepref_definition arena_length_impl 
+  is "uncurry (RETURN oo arena_length)" 
+    :: "[uncurry arena_is_valid_clause_idx]\<^sub>a arena_fast_assn\<^sup>k *\<^sub>a sint64_nat_assn\<^sup>k \<rightarrow> snat_assn' TYPE(64)"
+  unfolding arena_length_alt
+  supply [simp] = max_snat_def max_unat_def arena_length_impl_bounds_aux1
+    and [dest] = arena_lengthI
+  by sepref
+lemmas [sepref_fr_rules] = arena_length_impl.refine
+
+
+paragraph \<open>Literal at given position\<close>
+
+lemma arena_lit_implI:
+  assumes "arena_lit_pre a b"
+  shows "b < length a" "is_Lit (a ! b)"
+  using assms unfolding arena_lit_pre_def arena_is_valid_clause_idx_and_access_def
+  by (fastforce dest: arena_lifting)+
+
+sepref_register arena_lit xarena_lit
+sepref_definition arena_lit_impl 
+  is "uncurry (RETURN oo arena_lit)" 
+    :: "[uncurry arena_lit_pre]\<^sub>a arena_fast_assn\<^sup>k *\<^sub>a sint64_nat_assn\<^sup>k \<rightarrow> unat_lit_assn"
+  supply [intro] = arena_lit_implI
+  unfolding arena_lit_def
+  by sepref
+lemmas [sepref_fr_rules] = arena_lit_impl.refine
+
+      
+paragraph \<open>Status of the clause\<close>
+
+lemma arena_status_implI:
+  assumes "arena_is_valid_clause_vdom a b"
+  shows "4 \<le> b" "b - 4 < length a" "is_Status (a ! (b-4))"
+  using assms STATUS_SHIFT_def arena_dom_status_iff
+  unfolding arena_is_valid_clause_vdom_def
+  by (auto dest: valid_arena_in_vdom_le_arena)
+
+sepref_register arena_status xarena_status
+sepref_definition arena_status_impl 
+  is "uncurry (RETURN oo arena_status)" 
+    :: "[uncurry arena_is_valid_clause_vdom]\<^sub>a arena_fast_assn\<^sup>k *\<^sub>a sint64_nat_assn\<^sup>k \<rightarrow> status_impl_assn"
+  supply [intro] = arena_status_implI
+  supply [simp] = max_snat_def
+  unfolding arena_status_def STATUS_SHIFT_def
+  apply (annot_snat_const "TYPE(64)")
+  by sepref
+lemmas [sepref_fr_rules] = arena_status_impl.refine
+
+
+paragraph \<open>Swap literals\<close>
+sepref_register swap_lits
 sepref_definition swap_lits_impl is "uncurry3 (RETURN oooo swap_lits)"
-  :: "[\<lambda>(((C,i),j),arena). C + i < length arena \<and> C + j < length arena]\<^sub>a sint64_nat_assn\<^sup>k *\<^sub>a sint64_nat_assn\<^sup>k *\<^sub>a sint64_nat_assn\<^sup>k *\<^sub>a arena_assn\<^sup>d \<rightarrow> arena_assn"
+  :: "[\<lambda>(((C,i),j),arena). C + i < length arena \<and> C + j < length arena]\<^sub>a sint64_nat_assn\<^sup>k *\<^sub>a sint64_nat_assn\<^sup>k *\<^sub>a sint64_nat_assn\<^sup>k *\<^sub>a arena_fast_assn\<^sup>d \<rightarrow> arena_fast_assn"
   unfolding swap_lits_def convert_swap
   supply [dest] = rdomp_al_imp_len_bound
   unfolding swap_unfold
   by sepref
 
+lemmas [sepref_fr_rules] = swap_lits_impl.refine
+  
 paragraph \<open>Get LBD\<close>
-
-lemma xarena_lbd_refine1: "(\<lambda>eli. eli, xarena_lbd) \<in> [is_LBD]\<^sub>f arena_el_rel \<rightarrow> nat_rel"
-  by (auto intro!: frefI simp: arena_el_rel_def split: arena_el.splits)
-
-sepref_definition xarena_lbd_impl is "RETURN o (\<lambda>eli. eli)" :: "uint32_nat_assn\<^sup>k \<rightarrow>\<^sub>a uint32_nat_assn"
-  by sepref
-
-lemmas [sepref_fr_rules] = xarena_len_impl.refine[FCOMP xarena_lbd_refine1]
 
 lemma get_clause_LBD_preI:
   assumes "get_clause_LBD_pre a b"
@@ -174,27 +258,19 @@ lemma get_clause_LBD_preI:
   using LBD_SHIFT_def assms
   by (auto simp: get_clause_LBD_pre_def arena_is_valid_clause_idx_def arena_lifting)
 
-definition get_clause_LBD :: \<open>arena \<Rightarrow> nat \<Rightarrow> nat\<close> where
-  \<open>get_clause_LBD arena C =  xarena_lbd (arena ! (C - LBD_SHIFT))\<close>
-
+sepref_register arena_lbd
 sepref_definition arena_lbd_impl
-  is "uncurry (RETURN oo get_clause_LBD)"
-    :: "[uncurry get_clause_LBD_pre]\<^sub>a arena_assn\<^sup>k *\<^sub>a sint64_nat_assn\<^sup>k \<rightarrow>uint32_nat_assn"
-  unfolding get_clause_LBD_def LBD_SHIFT_def
+  is "uncurry (RETURN oo arena_lbd)"
+    :: "[uncurry get_clause_LBD_pre]\<^sub>a arena_fast_assn\<^sup>k *\<^sub>a sint64_nat_assn\<^sup>k \<rightarrow>uint32_nat_assn"
+  unfolding arena_lbd_def LBD_SHIFT_def
   supply [simp] = max_snat_def max_unat_def
     and [dest] = get_clause_LBD_preI
   apply (annot_snat_const "TYPE(64)")
   by sepref
+lemmas [sepref_fr_rules] = arena_lbd_impl.refine
 
-paragraph \<open>Get LBD\<close>
+paragraph \<open>Get Saved Position\<close>
 
-lemma xarena_pos_refine1: "(\<lambda>eli. eli, xarena_pos) \<in> [is_Pos]\<^sub>f arena_el_rel \<rightarrow> nat_rel"
-  by (auto intro!: frefI simp: arena_el_rel_def split: arena_el.splits)
-
-sepref_definition xarena_pos_impl is "RETURN o (\<lambda>eli. eli)" :: "uint32_nat_assn\<^sup>k \<rightarrow>\<^sub>a uint32_nat_assn"
-  by sepref
-
-lemmas [sepref_fr_rules] = xarena_len_impl.refine[FCOMP xarena_pos_refine1]
 
 lemma arena_posI:
   assumes "get_saved_pos_pre a b"
@@ -213,24 +289,17 @@ lemma arena_pos_alt:
     in snat_const TYPE(64) 2 + op_unat_snat_upcast TYPE(64) l)\<close>
   by (simp add: arena_pos_def POS_SHIFT_def)  
 
-
+sepref_register arena_pos
 sepref_definition arena_pos_impl 
   is "uncurry (RETURN oo arena_pos)" 
-    :: "[uncurry get_saved_pos_pre]\<^sub>a arena_assn\<^sup>k *\<^sub>a sint64_nat_assn\<^sup>k \<rightarrow> snat_assn' TYPE(64)"
+    :: "[uncurry get_saved_pos_pre]\<^sub>a arena_fast_assn\<^sup>k *\<^sub>a sint64_nat_assn\<^sup>k \<rightarrow> snat_assn' TYPE(64)"
   unfolding arena_pos_alt
   supply [simp] = max_snat_def max_unat_def arena_length_impl_bounds_aux1
     and [dest] = arena_posI
   by sepref
+lemmas [sepref_fr_rules] = arena_pos_impl.refine
 
 paragraph \<open>Update LBD\<close>
-
-lemma ALBD_refine1: "(\<lambda>eli. eli, ALBD) \<in> nat_rel \<rightarrow> arena_el_rel"
-  by (auto intro!: frefI simp: arena_el_rel_def split: arena_el.splits)
-
-sepref_definition xarena_ALBD_impl is "RETURN o (\<lambda>eli. eli)" :: "uint32_nat_assn\<^sup>k \<rightarrow>\<^sub>a uint32_nat_assn"
-  by sepref
-
-lemmas [sepref_fr_rules] = xarena_ALBD_impl.refine[FCOMP ALBD_refine1]
 
 lemma update_lbdI:
   assumes "update_lbd_pre ((b, lbd), a)"
@@ -241,1296 +310,215 @@ lemma update_lbdI:
     dest: arena_lifting(10))
   by (simp add: less_imp_diff_less valid_arena_def)
 
-(* TODO: Let monadify-phase do this automatically? trade-of: goal-size vs. lost information *) 
-
+sepref_register update_lbd
 sepref_definition update_lbd_impl 
   is "uncurry2 (RETURN ooo update_lbd)" 
-    :: "[update_lbd_pre]\<^sub>a sint64_nat_assn\<^sup>k *\<^sub>a uint32_nat_assn\<^sup>k *\<^sub>a arena_assn\<^sup>d  \<rightarrow> arena_assn"
+    :: "[update_lbd_pre]\<^sub>a sint64_nat_assn\<^sup>k *\<^sub>a uint32_nat_assn\<^sup>k *\<^sub>a arena_fast_assn\<^sup>d  \<rightarrow> arena_fast_assn"
   unfolding update_lbd_def LBD_SHIFT_def
   supply [simp] = max_snat_def max_unat_def arena_length_impl_bounds_aux1 update_lbdI
     and [dest] = arena_posI
   apply (annot_snat_const "TYPE(64)")
   by sepref
 
+lemmas [sepref_fr_rules] = update_lbd_impl.refine
+  
+  
 paragraph \<open>Update Saved Position\<close>
 
-(* TODO: converting from nat to uint32 is a little stupid and always useless (uint64 is enough everytime) *)
-definition isa_update_pos :: \<open>nat \<Rightarrow> nat \<Rightarrow> uint32 list \<Rightarrow> uint32 list nres\<close> where
-  \<open>isa_update_pos C n arena = do {
-      ASSERT(C - POS_SHIFT < length arena \<and> C \<ge> POS_SHIFT \<and> n \<ge> 2 \<and> n - 2 \<le> uint32_max);
-      RETURN (arena [C - POS_SHIFT := (uint32_of_nat (n - 2))])
-  }\<close>
+lemma update_posI:
+  assumes "isa_update_pos_pre ((b, pos), a)"
+  shows "5 \<le> b" "2 \<le> pos" "b-5 < length a"
+  using assms POS_SHIFT_def
+  unfolding isa_update_pos_pre_def
+  apply (auto simp: arena_is_valid_clause_idx_def arena_lifting)
+  (* TODO: Clean up this mess *)
+  apply (metis (full_types) MAX_LENGTH_SHORT_CLAUSE_def arena_is_valid_clause_idx_def arena_posI(1) get_saved_pos_pre_def)
+  by (simp add: less_imp_diff_less valid_arena_def)
+  
+lemma update_posI2:
+  assumes "isa_update_pos_pre ((b, pos), a)"
+  assumes "rdomp (al_assn arena_el_impl_assn) a"
+  shows "pos < 2 + max_unat 32"
+  using assms POS_SHIFT_def
+  unfolding isa_update_pos_pre_def
+  apply (auto simp: arena_is_valid_clause_idx_def arena_lifting)
+  sorry (* TODO !*)
+  
 
-definition arena_update_pos where
-  \<open>arena_update_pos C pos arena = arena[C - POS_SHIFT := APos (pos - 2)]\<close>
+sepref_register arena_update_pos   
+sepref_definition update_pos_impl
+  is "uncurry2 (RETURN ooo arena_update_pos)" 
+    :: "[isa_update_pos_pre]\<^sub>a sint64_nat_assn\<^sup>k *\<^sub>a sint64_nat_assn\<^sup>k *\<^sub>a arena_fast_assn\<^sup>d  \<rightarrow> arena_fast_assn"
+  unfolding arena_update_pos_def POS_SHIFT_def
+  apply (annot_snat_const "TYPE(64)")
+  apply (rewrite at "APos \<hole>" annot_snat_unat_downcast[where 'l=32])
+  supply [simp] = max_snat_def max_unat_def update_posI and [dest] = update_posI2
+  (*apply (rule hfref_with_rdomI)*)
+  by sepref
+lemmas [sepref_fr_rules] = update_pos_impl.refine
+  
+sepref_register IRRED LEARNED DELETED
+lemma IRRED_impl[sepref_import_param]: "(0,IRRED) \<in> status_impl_rel"
+  unfolding status_impl_rel_def status_rel_def unat_rel_def unat.rel_def
+  by (auto simp: in_br_conv)
+    
+lemma LEARNED_impl[sepref_import_param]: "(1,LEARNED) \<in> status_impl_rel"
+  unfolding status_impl_rel_def status_rel_def unat_rel_def unat.rel_def
+  by (auto simp: in_br_conv)
 
-lemma arena_update_pos_alt_def:
-  \<open>arena_update_pos C i N = update_pos_direct C (i - 2) N\<close>
-  by (auto simp: arena_update_pos_def update_pos_direct_def)
+lemma DELETED_impl[sepref_import_param]: "(3,DELETED) \<in> status_impl_rel"
+  unfolding status_impl_rel_def status_rel_def unat_rel_def unat.rel_def
+  by (auto simp: in_br_conv)
 
-lemma arena_update_pos_conv:
-  assumes
-    valid: \<open>valid_arena arena N x\<close> and
-    j: \<open>j \<in># dom_m N\<close> and
-    a: \<open>(a, arena) \<in> \<langle>uint32_nat_rel O arena_el_rel\<rangle>list_rel\<close> and
-    length: \<open>arena_length arena j > MAX_LENGTH_SHORT_CLAUSE\<close> and
-    pos_le: \<open>pos \<le> arena_length arena j\<close> and
-    b': \<open>pos \<ge> 2\<close>
-  shows
-    \<open>j - POS_SHIFT < length arena\<close> (is ?le) and
-    \<open>j \<ge> POS_SHIFT\<close> (is ?ge)
-    \<open>(a[j - POS_SHIFT := uint32_of_nat (pos - 2)], arena_update_pos j pos arena) \<in>
-      \<langle>uint32_nat_rel O arena_el_rel\<rangle>list_rel\<close> (is ?unat) and
-    \<open>pos - 2 \<le> uint32_max\<close>
-proof -
-  have j_le: \<open>j < length arena\<close> and
-    length: \<open>length (N \<propto> j) = arena_length arena j\<close> and
-    k1:\<open>\<And>k. k < length (N \<propto> j) \<Longrightarrow> N \<propto> j ! k = arena_lit arena (j + k)\<close> and
-    k2:\<open>\<And>k. k < length (N \<propto> j) \<Longrightarrow> is_Lit (arena ! (j+k))\<close> and
-    le: \<open>j + length (N \<propto> j) \<le> length arena\<close>  and
-    j_ge: \<open>header_size (N \<propto> j) \<le> j\<close> and
-    long: \<open>is_long_clause (N \<propto> j)\<close> and
-    pos: \<open>is_Pos (arena ! (j - POS_SHIFT))\<close> and
-    is_size: \<open>is_Size (arena ! (j - SIZE_SHIFT))\<close>
-    using arena_lifting[OF valid j] length by (auto simp: is_short_clause_def header_size_def)
-  show le': ?le and ?ge
-    using le j_ge long unfolding length[symmetric] header_size_def
-    by (auto split: if_splits simp: POS_SHIFT_def)
-  have
-    \<open>(a ! (j - SIZE_SHIFT),
-         (arena ! (j - SIZE_SHIFT)))
-       \<in> uint32_nat_rel O arena_el_rel\<close>
-    by (rule param_nth[OF _ _ a]) (use j_le in auto)
-  then show \<open>pos - 2 \<le> uint32_max\<close>
-    using b' length is_size pos_le nat_of_uint32_le_uint32_max[of \<open>a ! (j - SIZE_SHIFT)\<close>]
-    by (cases \<open>arena ! (j - SIZE_SHIFT)\<close>)
-      (auto simp: uint32_nat_rel_def br_def arena_el_rel_def arena_length_def)
-  then show ?unat
-    using length a pos b'
-      valid_arena_update_pos[OF valid j \<open>is_long_clause (N \<propto> j)\<close> ]
-    by (auto simp: arena_el_rel_def unat_lit_rel_def arena_lit_def arena_update_pos_def
-        uint32_nat_rel_def br_def Collect_eq_comp nat_of_uint32_notle_minus
-        nat_of_uint32_uint32_of_nat_id
-       split: arena_el.splits
-       intro!: list_rel_update')
-qed
+  
+lemma mark_garbageI:
+  assumes "mark_garbage_pre (a, b)"
+  shows "4 \<le> b" "b-4 < length a"
+  using assms STATUS_SHIFT_def
+  unfolding mark_garbage_pre_def
+  apply (auto simp: arena_is_valid_clause_idx_def arena_lifting)
+  apply (metis (full_types) arena_dom_status_iff(5) insertCI valid_arena_extra_information_mark_to_delete)
+  by (simp add: less_imp_diff_less valid_arena_def)
 
-
-lemma isa_update_pos:
-  \<open>(uncurry2 isa_update_pos, uncurry2 (RETURN ooo arena_update_pos)) \<in>
-    [isa_update_pos_pre]\<^sub>f
-     nat_rel \<times>\<^sub>f nat_rel \<times>\<^sub>f \<langle>uint32_nat_rel O arena_el_rel\<rangle>list_rel \<rightarrow>
-    \<langle>\<langle>uint32_nat_rel O arena_el_rel\<rangle>list_rel\<rangle>nres_rel\<close>
-  unfolding isa_arena_status_def arena_status_def
-  by (intro frefI nres_relI)
-    (auto simp: arena_is_valid_clause_idx_def uint64_nat_rel_def br_def two_uint64_def
-        list_rel_imp_same_length arena_length_uint64_conv arena_lifting
-        arena_is_valid_clause_idx_and_access_def arena_lbd_conv
-        arena_is_valid_clause_vdom_def arena_status_literal_conv
-        update_lbd_pre_def isa_update_pos_def update_pos_direct_def isa_update_pos_pre_def
-        isa_arena_swap_def swap_lits_def swap_lits_pre_def isa_update_lbd_def
-        arena_update_pos_conv
-      intro!: ASSERT_refine_left)
-
-
-paragraph \<open>Mark clause as garbage\<close>
-
-
-definition mark_garbage where
-  \<open>mark_garbage arena C = do {
-    ASSERT(C \<ge> STATUS_SHIFT \<and> C - STATUS_SHIFT < length arena);
-    RETURN (arena[C - STATUS_SHIFT := (3 :: uint32)])
-  }\<close>
-
-lemma mark_garbage_pre:
-  assumes
-    j: \<open>j \<in># dom_m N\<close> and
-    valid: \<open>valid_arena arena N x\<close> and
-    arena: \<open>(a, arena) \<in> \<langle>uint32_nat_rel O arena_el_rel\<rangle>list_rel\<close>
-  shows
-    \<open>STATUS_SHIFT \<le> j\<close> (is ?ge) and
-    \<open>(a[j - STATUS_SHIFT := 3], arena[j - STATUS_SHIFT := AStatus DELETED False])
-         \<in> \<langle>uint32_nat_rel O arena_el_rel\<rangle>list_rel\<close> (is ?rel) and
-    \<open>j - STATUS_SHIFT < length arena\<close> (is ?le)
-proof -
-  have j_le: \<open>j < length arena\<close> and
-    length: \<open>length (N \<propto> j) = arena_length arena j\<close> and
-    k1:\<open>\<And>k. k < length (N \<propto> j) \<Longrightarrow> N \<propto> j ! k = arena_lit arena (j + k)\<close> and
-    k2:\<open>\<And>k. k < length (N \<propto> j) \<Longrightarrow> is_Lit (arena ! (j+k))\<close> and
-    le: \<open>j + length (N \<propto> j) \<le> length arena\<close>  and
-    j_ge: \<open>header_size (N \<propto> j) \<le> j\<close>
-    using arena_lifting[OF valid j] by (auto simp: )
-  show le': ?le
-     using le j_ge unfolding length[symmetric] header_size_def
-     by (auto split: if_splits simp: SHIFTS_def)
-
-  show ?rel
-     apply (rule list_rel_update'[OF arena])
-     using length
-     by
-      (auto simp: arena_el_rel_def unat_lit_rel_def arena_lit_def update_lbd_def
-        uint32_nat_rel_def br_def Collect_eq_comp status_rel_def bitfield_rel_def
-       split: arena_el.splits
-       intro!: )
-  show ?ge
-    using le j_ge unfolding length[symmetric] header_size_def
-    by (auto split: if_splits simp: SHIFTS_def)
-qed
-
-lemma isa_mark_garbage:
-  \<open>(uncurry mark_garbage, uncurry (RETURN oo extra_information_mark_to_delete)) \<in>
-    [mark_garbage_pre]\<^sub>f
-     \<langle>uint32_nat_rel O arena_el_rel\<rangle>list_rel \<times>\<^sub>f nat_rel  \<rightarrow>
-    \<langle>\<langle>uint32_nat_rel O arena_el_rel\<rangle>list_rel\<rangle>nres_rel\<close>
-  unfolding isa_arena_status_def arena_status_def
-  by (intro frefI nres_relI)
-    (auto simp: arena_is_valid_clause_idx_def uint64_nat_rel_def br_def two_uint64_def
-        list_rel_imp_same_length arena_length_uint64_conv arena_lifting
-        arena_is_valid_clause_idx_and_access_def arena_lbd_conv
-        arena_is_valid_clause_vdom_def arena_status_literal_conv mark_garbage_pre
-        mark_garbage_def mark_garbage_pre_def extra_information_mark_to_delete_def
-        isa_arena_swap_def swap_lits_def swap_lits_pre_def isa_update_lbd_def
-      intro!: ASSERT_refine_left)
+sepref_register extra_information_mark_to_delete      
+sepref_definition mark_garbage_impl is "uncurry (RETURN oo extra_information_mark_to_delete)" 
+  :: "[mark_garbage_pre]\<^sub>a arena_fast_assn\<^sup>d *\<^sub>a sint64_nat_assn\<^sup>k \<rightarrow> arena_fast_assn"
+  unfolding extra_information_mark_to_delete_def STATUS_SHIFT_def
+  apply (annot_snat_const "TYPE(64)")
+  supply [simp] = max_snat_def mark_garbageI
+  by sepref
+lemmas [sepref_fr_rules] = mark_garbage_impl.refine
+  
 
 
 paragraph \<open>Activity\<close>
 
+lemma arena_act_implI:
+  assumes "arena_act_pre a b"
+  shows "3 \<le> b" "b - 3 < length a" "is_Act (a ! (b-3))"
+  using assms ACTIVITY_SHIFT_def 
+  apply (auto simp: arena_act_pre_def arena_is_valid_clause_idx_def arena_lifting)
+  by (simp add: less_imp_diff_less valid_arena_def)
+  
+sepref_register arena_act
+sepref_definition arena_act_impl 
+  is "uncurry (RETURN oo arena_act)" 
+    :: "[uncurry arena_act_pre]\<^sub>a arena_fast_assn\<^sup>k *\<^sub>a sint64_nat_assn\<^sup>k \<rightarrow> uint32_nat_assn"
+  supply [intro] = arena_act_implI
+  supply [simp] = max_snat_def
+  unfolding arena_act_def ACTIVITY_SHIFT_def
+  apply (annot_snat_const "TYPE(64)")
+  by sepref
+lemmas [sepref_fr_rules] = arena_act_impl.refine
 
-definition isa_arena_act :: \<open>uint32 list \<Rightarrow> nat \<Rightarrow> uint32 nres\<close> where
-  \<open>isa_arena_act arena C = do {
-      ASSERT(C - ACTIVITY_SHIFT < length arena \<and> C \<ge> ACTIVITY_SHIFT);
-      RETURN (arena ! (C - ACTIVITY_SHIFT))
-  }\<close>
-
-lemma arena_act_conv:
-  assumes
-    valid: \<open>valid_arena arena N x\<close> and
-    j: \<open>j \<in># dom_m N\<close> and
-    a: \<open>(a, arena) \<in> \<langle>uint32_nat_rel O arena_el_rel\<rangle>list_rel\<close>
-  shows
-    \<open>j - ACTIVITY_SHIFT < length arena\<close> (is ?le) and
-    \<open>ACTIVITY_SHIFT \<le> j\<close> (is ?ge) and
-    \<open>(a ! (j - ACTIVITY_SHIFT),
-        xarena_act (arena ! (j - ACTIVITY_SHIFT)))
-       \<in> uint32_nat_rel\<close>
-proof -
-  have j_le: \<open>j < length arena\<close> and
-    length: \<open>length (N \<propto> j) = arena_length arena j\<close> and
-    k1:\<open>\<And>k. k < length (N \<propto> j) \<Longrightarrow> N \<propto> j ! k = arena_lit arena (j + k)\<close> and
-    k2:\<open>\<And>k. k < length (N \<propto> j) \<Longrightarrow> is_Lit (arena ! (j+k))\<close> and
-    le: \<open>j + length (N \<propto> j) \<le> length arena\<close>  and
-    j_ge: \<open>header_size (N \<propto> j) \<le> j\<close> and
-    lbd: \<open>is_Act (arena ! (j - ACTIVITY_SHIFT))\<close>
-    using arena_lifting[OF valid j] by auto
-  show le': ?le
-     using le j_ge unfolding length[symmetric] header_size_def
-     by (auto split: if_splits simp: ACTIVITY_SHIFT_def)
-  show ?ge
-    using j_ge by (auto simp: SHIFTS_def header_size_def split: if_splits)
-  have
-    \<open>(a ! (j - ACTIVITY_SHIFT),
-         (arena ! (j - ACTIVITY_SHIFT)))
-       \<in> uint32_nat_rel O arena_el_rel\<close>
-    by (rule param_nth[OF _ _ a]) (use j_le in auto)
-  then show \<open>(a ! (j - ACTIVITY_SHIFT),
-        xarena_act (arena ! (j - ACTIVITY_SHIFT)))
-       \<in> uint32_nat_rel\<close>
-    using lbd by (cases \<open>arena ! (j - ACTIVITY_SHIFT)\<close>) (auto simp: arena_el_rel_def)
-qed
-
-lemma isa_arena_act_arena_act:
-  \<open>(uncurry isa_arena_act, uncurry (RETURN oo arena_act)) \<in>
-    [uncurry arena_act_pre]\<^sub>f
-     \<langle>uint32_nat_rel O arena_el_rel\<rangle>list_rel \<times>\<^sub>f nat_rel \<rightarrow>
-    \<langle>uint32_nat_rel\<rangle>nres_rel\<close>
-  by (intro frefI nres_relI)
-    (auto simp: isa_arena_act_def arena_act_def arena_get_lbd_conv
-      arena_act_pre_def arena_is_valid_clause_idx_def
-      list_rel_imp_same_length arena_act_conv
-      intro!: ASSERT_leI)
 
 
 paragraph \<open>Increment Activity\<close>
 
-definition isa_arena_incr_act :: \<open>uint32 list \<Rightarrow> nat \<Rightarrow> uint32 list nres\<close> where
-  \<open>isa_arena_incr_act arena C = do {
-      ASSERT(C - ACTIVITY_SHIFT < length arena \<and> C \<ge> ACTIVITY_SHIFT);
-      let act = arena ! (C - ACTIVITY_SHIFT);
-      RETURN (arena[C - ACTIVITY_SHIFT := act + 1])
-  }\<close>
+context begin                                             
 
-definition arena_incr_act where
-  \<open>arena_incr_act arena i = arena[i - ACTIVITY_SHIFT := AActivity (sum_mod_uint32_max 1 (xarena_act (arena!(i - ACTIVITY_SHIFT))))]\<close>
+interpretation llvm_prim_arith_setup .
 
-lemma arena_incr_act_conv:
-  assumes
-    valid: \<open>valid_arena arena N x\<close> and
-    j: \<open>j \<in># dom_m N\<close> and
-    a: \<open>(a, arena) \<in> \<langle>uint32_nat_rel O arena_el_rel\<rangle>list_rel\<close>
-  shows
-    \<open>j - ACTIVITY_SHIFT < length arena\<close> (is ?le) and
-    \<open>ACTIVITY_SHIFT \<le> j\<close> (is ?ge) and
-    \<open>(a[j - ACTIVITY_SHIFT := a ! (j - ACTIVITY_SHIFT) + 1], arena_incr_act arena j) \<in> \<langle>uint32_nat_rel O arena_el_rel\<rangle>list_rel\<close>
-proof -
-  have j_le: \<open>j < length arena\<close> and
-    length: \<open>length (N \<propto> j) = arena_length arena j\<close> and
-    k1:\<open>\<And>k. k < length (N \<propto> j) \<Longrightarrow> N \<propto> j ! k = arena_lit arena (j + k)\<close> and
-    k2:\<open>\<And>k. k < length (N \<propto> j) \<Longrightarrow> is_Lit (arena ! (j+k))\<close> and
-    le: \<open>j + length (N \<propto> j) \<le> length arena\<close>  and
-    j_ge: \<open>header_size (N \<propto> j) \<le> j\<close> and
-    lbd: \<open>is_Act (arena ! (j - ACTIVITY_SHIFT))\<close>
-    using arena_lifting[OF valid j] by auto
-  show le': ?le
-     using le j_ge unfolding length[symmetric] header_size_def
-     by (auto split: if_splits simp: ACTIVITY_SHIFT_def)
-  show ?ge
-    using j_ge by (auto simp: SHIFTS_def header_size_def split: if_splits)
-  have b:
-    \<open>(a ! (j - ACTIVITY_SHIFT),
-         (arena ! (j - ACTIVITY_SHIFT)))
-       \<in> uint32_nat_rel O arena_el_rel\<close>
-    by (rule param_nth[OF _ _ a]) (use j_le in auto)
-  show \<open>(a[j - ACTIVITY_SHIFT := a ! (j - ACTIVITY_SHIFT) + 1], arena_incr_act arena j) \<in> \<langle>uint32_nat_rel O arena_el_rel\<rangle>list_rel\<close>
-    unfolding arena_incr_act_def
-    by (rule list_rel_update'[OF a])
-      (cases \<open>arena ! (j - ACTIVITY_SHIFT)\<close>;
-      use lbd b in \<open>auto simp add: uint32_nat_rel_def br_def arena_el_rel_def
-        Collect_eq_comp sum_mod_uint32_max_def nat_of_uint32_plus\<close>)
-qed
+sepref_register op_incr_mod32
+lemma op_incr_mod32_hnr[sepref_fr_rules]: 
+  "(\<lambda>x. ll_add x 1, RETURN o op_incr_mod32) \<in> uint32_nat_assn\<^sup>k \<rightarrow>\<^sub>a uint32_nat_assn"
+  unfolding unat_rel_def unat.rel_def 
+  apply sepref_to_hoare
+  apply (simp add: in_br_conv)
+  apply vcg'
+  unfolding op_incr_mod32_def
+  by (simp add: unat_word_ariths)
 
+end  
+  
+sepref_register arena_incr_act
+sepref_definition arena_incr_act_impl is "uncurry (RETURN oo arena_incr_act)" 
+  :: "[uncurry arena_act_pre]\<^sub>a arena_fast_assn\<^sup>d *\<^sub>a sint64_nat_assn\<^sup>k \<rightarrow> arena_fast_assn"
+  unfolding arena_incr_act_def ACTIVITY_SHIFT_def
+  supply [intro] = arena_act_implI
+  supply [simp] = max_snat_def
+  apply (annot_snat_const "TYPE(64)")
+  by sepref
+lemmas [sepref_fr_rules] = arena_incr_act_impl.refine
 
-lemma isa_arena_incr_act_arena_incr_act:
-  \<open>(uncurry isa_arena_incr_act, uncurry (RETURN oo arena_incr_act)) \<in>
-    [uncurry arena_act_pre]\<^sub>f
-     \<langle>uint32_nat_rel O arena_el_rel\<rangle>list_rel \<times>\<^sub>f nat_rel \<rightarrow>
-    \<langle> \<langle>uint32_nat_rel O arena_el_rel\<rangle>list_rel\<rangle>nres_rel\<close>
-  by (intro frefI nres_relI)
-   (auto simp: isa_arena_incr_act_def arena_act_def arena_get_lbd_conv
-      arena_act_pre_def arena_is_valid_clause_idx_def arena_incr_act_conv
-      list_rel_imp_same_length arena_act_conv
-      intro!: ASSERT_leI)
-
-lemma length_arena_incr_act[simp]:
-  \<open>length (arena_incr_act arena C) = length arena\<close>
-  by (auto simp: arena_incr_act_def)
-
-lemma valid_arena_arena_incr_act:
-  assumes C: \<open>C \<in># dom_m N\<close> and valid: \<open>valid_arena arena N vdom\<close>
-  shows
-   \<open>valid_arena (arena_incr_act arena C) N vdom\<close>
-proof -
-  let ?arena = \<open>arena_incr_act arena C\<close>
-  have act: \<open>\<forall>i\<in>#dom_m N.
-     i < length (arena) \<and>
-     header_size (N \<propto> i) \<le> i \<and>
-     xarena_active_clause (clause_slice arena N i)
-      (the (fmlookup N i))\<close> and
-    dead: \<open>\<And>i. i \<in> vdom \<Longrightarrow> i \<notin># dom_m N \<Longrightarrow> i < length arena \<and>
-           4 \<le> i \<and> arena_dead_clause (Misc.slice (i - 4) i arena)\<close> and
-    C_ge: \<open>header_size (N \<propto> C) \<le> C\<close> and
-    C_le: \<open>C < length arena\<close> and
-    C_act: \<open>xarena_active_clause (clause_slice arena N C)
-      (the (fmlookup N C))\<close>
-    using assms
-    by (auto simp: valid_arena_def)
-  have
-   [simp]: \<open>clause_slice ?arena N C ! (header_size (N \<propto> C) - LBD_SHIFT) =
-           clause_slice arena N C ! (header_size (N \<propto> C) - LBD_SHIFT)\<close> and
-   [simp]: \<open>clause_slice ?arena N C ! (header_size (N \<propto> C) - STATUS_SHIFT) =
-           clause_slice arena N C ! (header_size (N \<propto> C) - STATUS_SHIFT)\<close> and
-   [simp]: \<open>clause_slice ?arena N C ! (header_size (N \<propto> C) - SIZE_SHIFT) =
-           clause_slice arena N C ! (header_size (N \<propto> C) - SIZE_SHIFT)\<close> and
-   [simp]: \<open>is_long_clause (N \<propto> C) \<Longrightarrow> clause_slice ?arena N C ! (header_size (N \<propto> C) - POS_SHIFT) =
-           clause_slice arena N C ! (header_size (N \<propto> C) - POS_SHIFT)\<close> and
-   [simp]: \<open>length (clause_slice  ?arena N C) = length (clause_slice arena N C)\<close> and
-   [simp]: \<open>is_Act (clause_slice ?arena N C ! (header_size (N \<propto> C) - ACTIVITY_SHIFT))\<close> and
-   [simp]: \<open>Misc.slice C (C + length (N \<propto> C)) ?arena =
-     Misc.slice C (C + length (N \<propto> C)) arena\<close>
-    using C_le C_ge unfolding SHIFTS_def arena_incr_act_def header_size_def
-    by (auto simp: Misc.slice_def drop_update_swap split: if_splits)
-
-  have \<open>xarena_active_clause (clause_slice ?arena N C) (the (fmlookup N C))\<close>
-    using C_act C_le C_ge unfolding xarena_active_clause_alt_def
-    by simp
-
-  then have 1: \<open>xarena_active_clause (clause_slice arena N i) (the (fmlookup N i)) \<Longrightarrow>
-     xarena_active_clause (clause_slice (arena_incr_act arena C) N i) (the (fmlookup N i))\<close>
-    if \<open>i \<in># dom_m N\<close>
-    for i
-    using minimal_difference_between_valid_index[of N arena C i, OF act]
-      minimal_difference_between_valid_index[of N arena i C, OF act] assms
-      that C_ge
-    by (cases \<open>C < i\<close>; cases \<open>C > i\<close>)
-      (auto simp: arena_incr_act_def header_size_def ACTIVITY_SHIFT_def
-      split: if_splits)
-
-  have 2:
-    \<open>arena_dead_clause (Misc.slice (i - 4) i ?arena)\<close>
-    if \<open>i \<in> vdom\<close>\<open>i \<notin># dom_m N\<close>\<open>arena_dead_clause (Misc.slice (i - 4) i arena)\<close>
-    for i
-  proof -
-    have i_ge: \<open>i \<ge> 4\<close> \<open>i < length arena\<close>
-      using that valid unfolding valid_arena_def
-      by auto
-    show ?thesis
-      using dead[of i] that C_le C_ge
-      minimal_difference_between_invalid_index[OF valid, of C i]
-      minimal_difference_between_invalid_index2[OF valid, of C i]
-      by (cases \<open>C < i\<close>; cases \<open>C > i\<close>)
-        (auto simp: arena_incr_act_def header_size_def ACTIVITY_SHIFT_def C
-          split: if_splits)
-  qed
-  show ?thesis
-    using 1 2 valid
-    by (auto simp: valid_arena_def)
-qed
-
-
-paragraph \<open>Divide activity by two\<close>
-
-definition isa_arena_decr_act :: \<open>uint32 list \<Rightarrow> nat \<Rightarrow> uint32 list nres\<close> where
-  \<open>isa_arena_decr_act arena C = do {
-      ASSERT(C - ACTIVITY_SHIFT < length arena \<and> C \<ge> ACTIVITY_SHIFT);
-      let act = arena ! (C - ACTIVITY_SHIFT);
-      RETURN (arena[C - ACTIVITY_SHIFT := (act >> 1)])
-  }\<close>
-
-lemma arena_decr_act_conv:
-  assumes
-    valid: \<open>valid_arena arena N x\<close> and
-    j: \<open>j \<in># dom_m N\<close> and
-    a: \<open>(a, arena) \<in> \<langle>uint32_nat_rel O arena_el_rel\<rangle>list_rel\<close>
-  shows
-    \<open>j - ACTIVITY_SHIFT < length arena\<close> (is ?le) and
-    \<open>ACTIVITY_SHIFT \<le> j\<close> (is ?ge) and
-    \<open>(a[j - ACTIVITY_SHIFT := a ! (j - ACTIVITY_SHIFT) >> Suc 0], arena_decr_act arena j)
-       \<in> \<langle>uint32_nat_rel O arena_el_rel\<rangle>list_rel\<close>
-proof -
-  have j_le: \<open>j < length arena\<close> and
-    length: \<open>length (N \<propto> j) = arena_length arena j\<close> and
-    k1:\<open>\<And>k. k < length (N \<propto> j) \<Longrightarrow> N \<propto> j ! k = arena_lit arena (j + k)\<close> and
-    k2:\<open>\<And>k. k < length (N \<propto> j) \<Longrightarrow> is_Lit (arena ! (j+k))\<close> and
-    le: \<open>j + length (N \<propto> j) \<le> length arena\<close>  and
-    j_ge: \<open>header_size (N \<propto> j) \<le> j\<close> and
-    lbd: \<open>is_Act (arena ! (j - ACTIVITY_SHIFT))\<close>
-    using arena_lifting[OF valid j] by auto
-  show le': ?le
-     using le j_ge unfolding length[symmetric] header_size_def
-     by (auto split: if_splits simp: ACTIVITY_SHIFT_def)
-  show ?ge
-    using j_ge by (auto simp: SHIFTS_def header_size_def split: if_splits)
-  have b:
-    \<open>(a ! (j - ACTIVITY_SHIFT),
-         (arena ! (j - ACTIVITY_SHIFT)))
-       \<in> uint32_nat_rel O arena_el_rel\<close>
-    by (rule param_nth[OF _ _ a]) (use j_le in auto)
-  show \<open>(a[j - ACTIVITY_SHIFT := a ! (j - ACTIVITY_SHIFT) >> Suc 0], arena_decr_act arena j)
-      \<in> \<langle>uint32_nat_rel O arena_el_rel\<rangle>list_rel\<close>
-    unfolding arena_decr_act_def
-    by (rule list_rel_update'[OF a])
-      (cases \<open>arena ! (j - ACTIVITY_SHIFT)\<close>;
-      use lbd b in \<open>auto simp add: uint32_nat_rel_def br_def arena_el_rel_def
-        Collect_eq_comp sum_mod_uint32_max_def nat_of_uint32_plus
-	nat_of_uint32_shiftr\<close>)
-qed
-
-lemma isa_arena_decr_act_arena_decr_act:
-  \<open>(uncurry isa_arena_decr_act, uncurry (RETURN oo arena_decr_act)) \<in>
-    [uncurry arena_act_pre]\<^sub>f
-     \<langle>uint32_nat_rel O arena_el_rel\<rangle>list_rel \<times>\<^sub>f nat_rel \<rightarrow>
-    \<langle> \<langle>uint32_nat_rel O arena_el_rel\<rangle>list_rel\<rangle>nres_rel\<close>
-  by (intro frefI nres_relI)
-   (auto simp: isa_arena_decr_act_def arena_act_def arena_get_lbd_conv
-      arena_act_pre_def arena_is_valid_clause_idx_def arena_decr_act_conv
-      list_rel_imp_same_length arena_act_conv
-      intro!: ASSERT_leI)
-
-      
-lemma valid_arena_arena_decr_act:
-  assumes C: \<open>C \<in># dom_m N\<close> and valid: \<open>valid_arena arena N vdom\<close>
-  shows
-   \<open>valid_arena (arena_decr_act arena C) N vdom\<close>
-proof -
-  let ?arena = \<open>arena_decr_act arena C\<close>
-  have act: \<open>\<forall>i\<in>#dom_m N.
-     i < length (arena) \<and>
-     header_size (N \<propto> i) \<le> i \<and>
-     xarena_active_clause (clause_slice arena N i)
-      (the (fmlookup N i))\<close> and
-    dead: \<open>\<And>i. i \<in> vdom \<Longrightarrow> i \<notin># dom_m N \<Longrightarrow> i < length arena \<and>
-           4 \<le> i \<and> arena_dead_clause (Misc.slice (i - 4) i arena)\<close> and
-    C_ge: \<open>header_size (N \<propto> C) \<le> C\<close> and
-    C_le: \<open>C < length arena\<close> and
-    C_act: \<open>xarena_active_clause (clause_slice arena N C)
-      (the (fmlookup N C))\<close>
-    using assms
-    by (auto simp: valid_arena_def)
-  have
-   [simp]: \<open>clause_slice ?arena N C ! (header_size (N \<propto> C) - LBD_SHIFT) =
-           clause_slice arena N C ! (header_size (N \<propto> C) - LBD_SHIFT)\<close> and
-   [simp]: \<open>clause_slice ?arena N C ! (header_size (N \<propto> C) - STATUS_SHIFT) =
-           clause_slice arena N C ! (header_size (N \<propto> C) - STATUS_SHIFT)\<close> and
-   [simp]: \<open>clause_slice ?arena N C ! (header_size (N \<propto> C) - SIZE_SHIFT) =
-           clause_slice arena N C ! (header_size (N \<propto> C) - SIZE_SHIFT)\<close> and
-   [simp]: \<open>is_long_clause (N \<propto> C) \<Longrightarrow> clause_slice ?arena N C ! (header_size (N \<propto> C) - POS_SHIFT) =
-           clause_slice arena N C ! (header_size (N \<propto> C) - POS_SHIFT)\<close> and
-   [simp]: \<open>length (clause_slice  ?arena N C) = length (clause_slice arena N C)\<close> and
-   [simp]: \<open>is_Act (clause_slice ?arena N C ! (header_size (N \<propto> C) - ACTIVITY_SHIFT))\<close> and
-   [simp]: \<open>Misc.slice C (C + length (N \<propto> C)) ?arena =
-     Misc.slice C (C + length (N \<propto> C)) arena\<close>
-    using C_le C_ge unfolding SHIFTS_def arena_decr_act_def header_size_def
-    by (auto simp: Misc.slice_def drop_update_swap split: if_splits)
-
-  have \<open>xarena_active_clause (clause_slice ?arena N C) (the (fmlookup N C))\<close>
-    using C_act C_le C_ge unfolding xarena_active_clause_alt_def
-    by simp
-
-  then have 1: \<open>xarena_active_clause (clause_slice arena N i) (the (fmlookup N i)) \<Longrightarrow>
-     xarena_active_clause (clause_slice (arena_decr_act arena C) N i) (the (fmlookup N i))\<close>
-    if \<open>i \<in># dom_m N\<close>
-    for i
-    using minimal_difference_between_valid_index[of N arena C i, OF act]
-      minimal_difference_between_valid_index[of N arena i C, OF act] assms
-      that C_ge
-    by (cases \<open>C < i\<close>; cases \<open>C > i\<close>)
-      (auto simp: arena_decr_act_def header_size_def ACTIVITY_SHIFT_def
-      split: if_splits)
-
-  have 2:
-    \<open>arena_dead_clause (Misc.slice (i - 4) i ?arena)\<close>
-    if \<open>i \<in> vdom\<close>\<open>i \<notin># dom_m N\<close>\<open>arena_dead_clause (Misc.slice (i - 4) i arena)\<close>
-    for i
-  proof -
-    have i_ge: \<open>i \<ge> 4\<close> \<open>i < length arena\<close>
-      using that valid unfolding valid_arena_def
-      by auto
-    show ?thesis
-      using dead[of i] that C_le C_ge
-      minimal_difference_between_invalid_index[OF valid, of C i]
-      minimal_difference_between_invalid_index2[OF valid, of C i]
-      by (cases \<open>C < i\<close>; cases \<open>C > i\<close>)
-        (auto simp: arena_decr_act_def header_size_def ACTIVITY_SHIFT_def C
-          split: if_splits)
-  qed
-  show ?thesis
-    using 1 2 valid
-    by (auto simp: valid_arena_def)
-qed
+sepref_register arena_decr_act
+sepref_definition arena_decr_act_impl is "uncurry (RETURN oo arena_decr_act)" 
+  :: "[uncurry arena_act_pre]\<^sub>a arena_fast_assn\<^sup>d *\<^sub>a sint64_nat_assn\<^sup>k \<rightarrow> arena_fast_assn"
+  unfolding arena_decr_act_def ACTIVITY_SHIFT_def
+  supply [intro] = arena_act_implI
+  supply [simp] = max_snat_def max_unat_def
+  apply (rewrite at "_ div \<hole>"  unat_const_fold[where 'a=32])
+  apply (annot_snat_const "TYPE(64)")
+  by sepref
+lemmas [sepref_fr_rules] = arena_decr_act_impl.refine
 
 
 paragraph \<open>Mark used\<close>
 
-definition isa_mark_used :: \<open>uint32 list \<Rightarrow> nat \<Rightarrow> uint32 list nres\<close> where
-  \<open>isa_mark_used arena C = do {
-      ASSERT(C - STATUS_SHIFT < length arena \<and> C \<ge> STATUS_SHIFT);
-      let act = arena ! (C - STATUS_SHIFT);
-      RETURN (arena[C - STATUS_SHIFT := act OR 0b100])
-  }\<close>
+term mark_used
 
-lemma isa_mark_used_conv:
-  assumes
-    valid: \<open>valid_arena arena N x\<close> and
-    j: \<open>j \<in># dom_m N\<close> and
-    a: \<open>(a, arena) \<in> \<langle>uint32_nat_rel O arena_el_rel\<rangle>list_rel\<close>
-  shows
-    \<open>j - STATUS_SHIFT < length arena\<close> (is ?le) and
-    \<open>STATUS_SHIFT \<le> j\<close> (is ?ge) and
-    \<open>(a[j - STATUS_SHIFT := a ! (j - STATUS_SHIFT) OR 4], mark_used arena j) \<in> \<langle>uint32_nat_rel O arena_el_rel\<rangle>list_rel\<close>
-proof -
-  have j_le: \<open>j < length arena\<close> and
-    length: \<open>length (N \<propto> j) = arena_length arena j\<close> and
-    k1:\<open>\<And>k. k < length (N \<propto> j) \<Longrightarrow> N \<propto> j ! k = arena_lit arena (j + k)\<close> and
-    k2:\<open>\<And>k. k < length (N \<propto> j) \<Longrightarrow> is_Lit (arena ! (j+k))\<close> and
-    le: \<open>j + length (N \<propto> j) \<le> length arena\<close>  and
-    j_ge: \<open>header_size (N \<propto> j) \<le> j\<close> and
-    lbd: \<open>is_Status (arena ! (j - STATUS_SHIFT))\<close>
-    using arena_lifting[OF valid j] by auto
-  show le': ?le
-     using le j_ge unfolding length[symmetric] header_size_def
-     by (auto split: if_splits simp: STATUS_SHIFT_def)
-  show ?ge
-    using j_ge by (auto simp: SHIFTS_def header_size_def split: if_splits)
-  have b:
-    \<open>(a ! (j - STATUS_SHIFT),
-         (arena ! (j - STATUS_SHIFT)))
-       \<in> uint32_nat_rel O arena_el_rel\<close>
-    by (rule param_nth[OF _ _ a]) (use j_le in auto)
-  have [simp]: \<open>(a OR 4) AND 3 = a AND 3\<close> for a :: int
-    supply [[show_types]]
-    by (smt BIT_special_simps(1) BIT_special_simps(4) One_nat_def bbw_ao_dist expand_BIT(2)
-      int_and_comm int_and_numerals(17) int_and_numerals(3) int_or_extra_simps(1)
-      numeral_One numeral_plus_one of_nat_numeral semiring_1_class.of_nat_simps(1)
-      semiring_1_class.of_nat_simps(2) semiring_norm(2) semiring_norm(8))
-  have Pos: \<open>b \<ge>0 \<Longrightarrow> a \<le> a OR b\<close> for a b :: int
-    by (rule le_int_or)
-      (auto simp: bin_sign_def)
-  have [simp]: \<open>(0::int) \<le> int a OR (4::int)\<close> for a :: nat
-    by (rule order_trans[OF _ Pos])
-      auto
-  then have [simp]: \<open>(a OR 4) AND 3 = a AND 3\<close> for a :: nat
-    supply [[show_types]]
-    unfolding bitAND_nat_def bitOR_nat_def
-    by auto
+lemma arena_mark_used_implI:
+  assumes "arena_act_pre a b"
+  shows "4 \<le> b" "b - 4 < length a" "is_Status (a ! (b-4))"
+  using assms STATUS_SHIFT_def 
+  apply (auto simp: arena_act_pre_def arena_is_valid_clause_idx_def arena_lifting)
+  subgoal by (metis (full_types) arena_is_valid_clause_vdom_def arena_status_implI(1) insertCI valid_arena_extra_information_mark_to_delete)
+  subgoal by (simp add: less_imp_diff_less valid_arena_def)
+  done
 
-  have [simp]: \<open>(a OR 4) AND 4 = 4\<close> for a :: nat
-    supply [[show_types]]
-    unfolding bitAND_nat_def bitOR_nat_def
-    by auto
-  have nat_of_uint32_4: \<open>4 = nat_of_uint32 4\<close>
-    by auto
-  have [simp]: \<open>nat_of_uint32 (a OR 4) = nat_of_uint32 a OR 4\<close> for a
-    by (subst nat_of_uint32_4, subst nat_of_uint32_ao) simp
+(* TODO: Wrong name for precondition! *)
+sepref_register mark_used
+sepref_definition mark_used_impl is "uncurry (RETURN oo mark_used)" 
+  :: "[uncurry arena_act_pre]\<^sub>a arena_fast_assn\<^sup>d *\<^sub>a sint64_nat_assn\<^sup>k \<rightarrow> arena_fast_assn"
+  unfolding mark_used_def STATUS_SHIFT_def
+  supply [intro] = arena_mark_used_implI
+  supply [simp] = max_snat_def max_unat_def
+  apply (annot_snat_const "TYPE(64)")
+  by sepref
+lemmas [sepref_fr_rules] = mark_used_impl.refine
 
-  show \<open>(a[j - STATUS_SHIFT := a ! (j - STATUS_SHIFT) OR 0b100],
-      mark_used arena j) \<in> \<langle>uint32_nat_rel O arena_el_rel\<rangle>list_rel\<close>
-    unfolding mark_used_def
-    by (rule list_rel_update'[OF a])
-      (cases \<open>arena ! (j - STATUS_SHIFT)\<close>;
-      use lbd b in \<open>auto simp add: uint32_nat_rel_def br_def arena_el_rel_def
-          status_rel_def bitfield_rel_def
-          Collect_eq_comp sum_mod_uint32_max_def nat_of_uint32_plus\<close>)
-qed
+sepref_register mark_unused
+sepref_definition mark_unused_impl is "uncurry (RETURN oo mark_unused)" 
+  :: "[uncurry arena_act_pre]\<^sub>a arena_fast_assn\<^sup>d *\<^sub>a sint64_nat_assn\<^sup>k \<rightarrow> arena_fast_assn"
+  unfolding mark_unused_def STATUS_SHIFT_def
+  supply [intro] = arena_mark_used_implI
+  supply [simp] = max_snat_def max_unat_def
+  apply (annot_snat_const "TYPE(64)")
+  by sepref
+lemmas [sepref_fr_rules] = mark_unused_impl.refine
 
-
-lemma isa_mark_used_mark_used:
-  \<open>(uncurry isa_mark_used, uncurry (RETURN oo mark_used)) \<in>
-    [uncurry arena_act_pre]\<^sub>f
-     \<langle>uint32_nat_rel O arena_el_rel\<rangle>list_rel \<times>\<^sub>f nat_rel \<rightarrow>
-    \<langle> \<langle>uint32_nat_rel O arena_el_rel\<rangle>list_rel\<rangle>nres_rel\<close>
-  by (intro frefI nres_relI)
-   (auto simp: isa_mark_used_def arena_get_lbd_conv
-      arena_act_pre_def arena_is_valid_clause_idx_def arena_incr_act_conv
-      list_rel_imp_same_length isa_mark_used_conv
-      intro!: ASSERT_leI)
  
-paragraph \<open>Mark unused\<close>
-
-definition isa_mark_unused :: \<open>uint32 list \<Rightarrow> nat \<Rightarrow> uint32 list nres\<close> where
-  \<open>isa_mark_unused arena C = do {
-      ASSERT(C - STATUS_SHIFT < length arena \<and> C \<ge> STATUS_SHIFT);
-      let act = arena ! (C - STATUS_SHIFT);
-      RETURN (arena[C - STATUS_SHIFT := act AND 0b11])
-  }\<close>
-
-lemma isa_mark_unused_conv:
-  assumes
-    valid: \<open>valid_arena arena N x\<close> and
-    j: \<open>j \<in># dom_m N\<close> and
-    a: \<open>(a, arena) \<in> \<langle>uint32_nat_rel O arena_el_rel\<rangle>list_rel\<close>
-  shows
-    \<open>j - STATUS_SHIFT < length arena\<close> (is ?le) and
-    \<open>STATUS_SHIFT \<le> j\<close> (is ?ge) and
-    \<open>(a[j - STATUS_SHIFT := a ! (j - STATUS_SHIFT) AND 3], mark_unused arena j) \<in> \<langle>uint32_nat_rel O arena_el_rel\<rangle>list_rel\<close>
-proof -
-  have j_le: \<open>j < length arena\<close> and
-    length: \<open>length (N \<propto> j) = arena_length arena j\<close> and
-    k1:\<open>\<And>k. k < length (N \<propto> j) \<Longrightarrow> N \<propto> j ! k = arena_lit arena (j + k)\<close> and
-    k2:\<open>\<And>k. k < length (N \<propto> j) \<Longrightarrow> is_Lit (arena ! (j+k))\<close> and
-    le: \<open>j + length (N \<propto> j) \<le> length arena\<close>  and
-    j_ge: \<open>header_size (N \<propto> j) \<le> j\<close> and
-    lbd: \<open>is_Status (arena ! (j - STATUS_SHIFT))\<close>
-    using arena_lifting[OF valid j] by auto
-  show le': ?le
-     using le j_ge unfolding length[symmetric] header_size_def
-     by (auto split: if_splits simp: STATUS_SHIFT_def)
-  show ?ge
-    using j_ge by (auto simp: SHIFTS_def header_size_def split: if_splits)
-  have b:
-    \<open>(a ! (j - STATUS_SHIFT),
-         (arena ! (j - STATUS_SHIFT)))
-       \<in> uint32_nat_rel O arena_el_rel\<close>
-    by (rule param_nth[OF _ _ a]) (use j_le in auto)
-  have [simp]: \<open>(a OR 4) AND 3 = a AND 3\<close> for a :: int
-    supply [[show_types]]
-    by (smt BIT_special_simps(1) BIT_special_simps(4) One_nat_def bbw_ao_dist expand_BIT(2)
-      int_and_comm int_and_numerals(17) int_and_numerals(3) int_or_extra_simps(1)
-      numeral_One numeral_plus_one of_nat_numeral semiring_1_class.of_nat_simps(1)
-      semiring_1_class.of_nat_simps(2) semiring_norm(2) semiring_norm(8))
-  have Pos: \<open>b \<ge>0 \<Longrightarrow> a \<le> a OR b\<close> for a b :: int
-    by (rule le_int_or)
-      (auto simp: bin_sign_def)
-  have [simp]: \<open>(0::int) \<le> int a OR (4::int)\<close> for a :: nat
-    by (rule order_trans[OF _ Pos])
-      auto
-  then have [simp]: \<open>(a OR 4) AND 3 = a AND 3\<close> for a :: nat
-    supply [[show_types]]
-    unfolding bitAND_nat_def bitOR_nat_def
-    by auto
-
-  have [simp]: \<open>(a OR 4) AND 4 = 4\<close> for a :: nat
-    supply [[show_types]]
-    unfolding bitAND_nat_def bitOR_nat_def
-    by auto
-  have nat_of_uint32_4: \<open>3 = nat_of_uint32 3\<close>
-    by auto
-  have [simp]: \<open>nat_of_uint32 (a AND 3) = nat_of_uint32 a AND 3\<close> for a
-    by (subst nat_of_uint32_4, subst nat_of_uint32_ao) simp
-  (* TODO mark nat_0_AND as [simp] *)
-  show \<open>(a[j - STATUS_SHIFT := a ! (j - STATUS_SHIFT) AND 3],
-      mark_unused arena j) \<in> \<langle>uint32_nat_rel O arena_el_rel\<rangle>list_rel\<close>
-    unfolding mark_unused_def
-    supply [[show_types]]
-    by (rule list_rel_update'[OF a])
-      (cases \<open>arena ! (j - STATUS_SHIFT)\<close>;
-      use lbd b in \<open>auto simp add: uint32_nat_rel_def br_def arena_el_rel_def
-          status_rel_def bitfield_rel_def nat_0_AND
-          Collect_eq_comp sum_mod_uint32_max_def nat_of_uint32_plus\<close>)
-qed
-
-
-lemma isa_mark_unused_mark_unused:
-  \<open>(uncurry isa_mark_unused, uncurry (RETURN oo mark_unused)) \<in>
-    [uncurry arena_act_pre]\<^sub>f
-     \<langle>uint32_nat_rel O arena_el_rel\<rangle>list_rel \<times>\<^sub>f nat_rel \<rightarrow>
-    \<langle> \<langle>uint32_nat_rel O arena_el_rel\<rangle>list_rel\<rangle>nres_rel\<close>
-  by (intro frefI nres_relI)
-   (auto simp: isa_mark_unused_def arena_get_lbd_conv
-      arena_act_pre_def arena_is_valid_clause_idx_def arena_incr_act_conv
-      list_rel_imp_same_length isa_mark_unused_conv
-      intro!: ASSERT_leI)
-
 
 paragraph \<open>Marked as used?\<close>
 
-definition isa_marked_as_used :: \<open>uint32 list \<Rightarrow> nat \<Rightarrow> bool nres\<close> where
-  \<open>isa_marked_as_used arena C = do {
-      ASSERT(C - STATUS_SHIFT < length arena \<and> C \<ge> STATUS_SHIFT);
-      RETURN (arena ! (C - STATUS_SHIFT) AND 4 \<noteq> 0)
-  }\<close>
+lemma arena_marked_as_used_implI:
+  assumes "marked_as_used_pre a b"
+  shows "4 \<le> b" "b - 4 < length a" "is_Status (a ! (b-4))"
+  using assms STATUS_SHIFT_def 
+  apply (auto simp: marked_as_used_pre_def arena_is_valid_clause_idx_def arena_lifting)
+  subgoal by (metis (full_types) arena_is_valid_clause_vdom_def arena_status_implI(1) insertCI valid_arena_extra_information_mark_to_delete)
+  subgoal by (simp add: less_imp_diff_less valid_arena_def)
+  done
 
-
-
-lemma arena_marked_as_used_conv:
-  assumes
-    valid: \<open>valid_arena arena N x\<close> and
-    j: \<open>j \<in># dom_m N\<close> and
-    a: \<open>(a, arena) \<in> \<langle>uint32_nat_rel O arena_el_rel\<rangle>list_rel\<close>
-  shows
-    \<open>j - STATUS_SHIFT < length arena\<close> (is ?le) and
-    \<open>STATUS_SHIFT \<le> j\<close> (is ?ge) and
-    \<open>a ! (j - STATUS_SHIFT) AND 4 \<noteq> 0 \<longleftrightarrow>
-        marked_as_used arena j\<close>
-proof -
-  have j_le: \<open>j < length arena\<close> and
-    length: \<open>length (N \<propto> j) = arena_length arena j\<close> and
-    k1: \<open>\<And>k. k < length (N \<propto> j) \<Longrightarrow> N \<propto> j ! k = arena_lit arena (j + k)\<close> and
-    k2: \<open>\<And>k. k < length (N \<propto> j) \<Longrightarrow> is_Lit (arena ! (j+k))\<close> and
-    le: \<open>j + length (N \<propto> j) \<le> length arena\<close>  and
-    j_ge: \<open>header_size (N \<propto> j) \<le> j\<close> and
-    lbd: \<open>is_Status (arena ! (j - STATUS_SHIFT))\<close>
-    using arena_lifting[OF valid j] by (auto simp: )
-  show le': ?le
-     using le j_ge unfolding length[symmetric] header_size_def
-     by (auto split: if_splits simp: STATUS_SHIFT_def)
-  show ?ge
-    using j_ge by (auto simp: SHIFTS_def header_size_def split: if_splits)
-  have [simp]: \<open>a \<noteq> 0 \<longleftrightarrow> nat_of_uint32 a \<noteq> 0\<close> for a:: uint32
-    by (simp add: nat_of_uint32_0_iff)
-  have
-    \<open>(a ! (j - STATUS_SHIFT),
-         (arena ! (j - STATUS_SHIFT)))
-       \<in> uint32_nat_rel O arena_el_rel\<close>
-    by (rule param_nth[OF _ _ a]) (use j_le in auto)
-  then show \<open>a ! (j - STATUS_SHIFT) AND 4 \<noteq> 0 \<longleftrightarrow>
-        marked_as_used arena j\<close>
-    using lbd by (cases \<open>arena ! (j - STATUS_SHIFT)\<close>)
-      (auto simp: arena_el_rel_def bitfield_rel_def nat_of_uint32_ao[symmetric]
-      marked_as_used_def uint32_nat_rel_def br_def)
-qed
-
-
-
-lemma isa_marked_as_used_marked_as_used:
-  \<open>(uncurry isa_marked_as_used, uncurry (RETURN oo marked_as_used)) \<in>
-    [uncurry marked_as_used_pre]\<^sub>f
-     \<langle>uint32_nat_rel O arena_el_rel\<rangle>list_rel \<times>\<^sub>f nat_rel \<rightarrow>
-    \<langle>bool_rel\<rangle>nres_rel\<close>
-  by (intro frefI nres_relI)
-    (auto simp: marked_as_used_pre_def arena_marked_as_used_conv
-      get_clause_LBD_pre_def arena_is_valid_clause_idx_def
-      list_rel_imp_same_length isa_marked_as_used_def
-      intro!: ASSERT_leI)
-
-abbreviation arena_el_assn :: "arena_el \<Rightarrow> uint32 \<Rightarrow> assn" where
-  \<open>arena_el_assn \<equiv> hr_comp uint32_nat_assn arena_el_rel\<close>
-
-abbreviation arena_assn :: "arena_el list \<Rightarrow> uint32 array_list \<Rightarrow> assn" where
-  \<open>arena_assn \<equiv> arl_assn arena_el_assn\<close>
-
-abbreviation arena_fast_assn :: "arena_el list \<Rightarrow> uint32 array_list64 \<Rightarrow> assn" where
-  \<open>arena_fast_assn \<equiv> arl64_assn arena_el_assn\<close>
-
-abbreviation status_assn where
-  \<open>status_assn \<equiv> hr_comp uint32_nat_assn status_rel\<close>
-
-abbreviation clause_status_assn where
-  \<open>clause_status_assn \<equiv> (id_assn :: clause_status \<Rightarrow> _)\<close>
-
-lemma IRRED_hnr[sepref_fr_rules]:
-  \<open>(uncurry0 (return IRRED), uncurry0 (RETURN IRRED)) \<in> unit_assn\<^sup>k \<rightarrow>\<^sub>a clause_status_assn\<close>
-  by sepref_to_hoare sep_auto
-
-lemma LEARNED_hnr[sepref_fr_rules]:
-  \<open>(uncurry0 (return LEARNED), uncurry0 (RETURN LEARNED)) \<in> unit_assn\<^sup>k \<rightarrow>\<^sub>a clause_status_assn\<close>
-  by sepref_to_hoare sep_auto
-
-lemma DELETED_hnr[sepref_fr_rules]:
-  \<open>(uncurry0 (return DELETED), uncurry0 (RETURN DELETED)) \<in> unit_assn\<^sup>k \<rightarrow>\<^sub>a clause_status_assn\<close>
-  by sepref_to_hoare sep_auto
-
-lemma ACTIVITY_SHIFT_hnr:
-  \<open>(uncurry0 (return 3), uncurry0 (RETURN ACTIVITY_SHIFT) ) \<in> unit_assn\<^sup>k \<rightarrow>\<^sub>a uint64_nat_assn\<close>
-  by sepref_to_hoare (sep_auto simp: ACTIVITY_SHIFT_def uint64_nat_rel_def br_def)
-lemma STATUS_SHIFT_hnr:
-  \<open>(uncurry0 (return 4), uncurry0 (RETURN STATUS_SHIFT) ) \<in> unit_assn\<^sup>k \<rightarrow>\<^sub>a uint64_nat_assn\<close>
-  by sepref_to_hoare (sep_auto simp: STATUS_SHIFT_def uint64_nat_rel_def br_def)
-
-lemma [sepref_fr_rules]:
-  \<open>(uncurry0 (return 1), uncurry0 (RETURN SIZE_SHIFT)) \<in> unit_assn\<^sup>k \<rightarrow>\<^sub>a nat_assn\<close>
-  by sepref_to_hoare (sep_auto simp: SIZE_SHIFT_def)
-
-lemma [sepref_fr_rules]:
-  \<open>(return o id, RETURN o xarena_length) \<in> [is_Size]\<^sub>a arena_el_assn\<^sup>k \<rightarrow> uint32_nat_assn\<close>
-  by sepref_to_hoare (sep_auto simp: SIZE_SHIFT_def uint32_nat_rel_def
-    arena_el_rel_def br_def hr_comp_def split: arena_el.splits)
-
-lemma (in -) POS_SHIFT_uint64_hnr:
-  \<open>(uncurry0 (return 5), uncurry0 (RETURN POS_SHIFT)) \<in> unit_assn\<^sup>k \<rightarrow>\<^sub>a uint64_nat_assn\<close>
-  by sepref_to_hoare (sep_auto simp: POS_SHIFT_def uint64_nat_rel_def br_def)
-
-lemma nat_of_uint64_eq_2_iff[simp]: \<open>nat_of_uint64 c = 2 \<longleftrightarrow> c = 2\<close>
-  using word_nat_of_uint64_Rep_inject by fastforce
-
-lemma arena_el_assn_alt_def:
-  \<open>arena_el_assn = hr_comp uint32_assn (uint32_nat_rel O arena_el_rel)\<close>
-  by (auto simp: hr_comp_assoc[symmetric])
-
-lemma arena_el_comp: \<open>hn_val (uint32_nat_rel O arena_el_rel) = hn_ctxt arena_el_assn\<close>
-  by (auto simp: hn_ctxt_def arena_el_assn_alt_def)
-
-lemma status_assn_hnr_eq[sepref_fr_rules]:
-  \<open>(uncurry (return oo (=)), uncurry (RETURN oo (=))) \<in> status_assn\<^sup>k *\<^sub>a status_assn\<^sup>k \<rightarrow>\<^sub>a
-    bool_assn\<close>
-  by sepref_to_hoare (sep_auto simp: status_rel_def hr_comp_def uint32_nat_rel_def br_def
-    nat_of_uint32_0_iff nat_of_uint32_Suc03_iff nat_of_uint32_013_neq)
-
-lemma IRRED_status_assn[sepref_fr_rules]:
-  \<open>(uncurry0 (return 0), uncurry0 (RETURN IRRED)) \<in> unit_assn\<^sup>k \<rightarrow>\<^sub>a status_assn\<close>
-  by (sepref_to_hoare) (sep_auto simp: status_rel_def hr_comp_def uint32_nat_rel_def br_def)
-
-lemma LEARNED_status_assn[sepref_fr_rules]:
-  \<open>(uncurry0 (return 1), uncurry0 (RETURN LEARNED)) \<in> unit_assn\<^sup>k \<rightarrow>\<^sub>a status_assn\<close>
-  by (sepref_to_hoare) (sep_auto simp: status_rel_def hr_comp_def uint32_nat_rel_def br_def)
-
-lemma DELETED_status_assn[sepref_fr_rules]:
-  \<open>(uncurry0 (return 3), uncurry0 (RETURN DELETED)) \<in> unit_assn\<^sup>k \<rightarrow>\<^sub>a status_assn\<close>
-  by (sepref_to_hoare) (sep_auto simp: status_rel_def hr_comp_def uint32_nat_rel_def br_def
-    nat_of_uint32_Suc03_iff)
-
-lemma status_assn_alt_def:
-  \<open>status_assn = pure (uint32_nat_rel O status_rel)\<close>
-  unfolding hr_comp_pure by simp
-
-lemma [sepref_fr_rules]:
-  \<open>(uncurry0 (return 2), uncurry0 (RETURN LBD_SHIFT)) \<in> unit_assn\<^sup>k \<rightarrow>\<^sub>a nat_assn\<close>
-  by sepref_to_hoare (sep_auto simp: LBD_SHIFT_def)
-
-lemma [sepref_fr_rules]:
-  \<open>(uncurry0 (return 4), uncurry0 (RETURN STATUS_SHIFT)) \<in> unit_assn\<^sup>k \<rightarrow>\<^sub>a nat_assn\<close>
-  by sepref_to_hoare (sep_auto simp: STATUS_SHIFT_def)
-
-lemma (in -) LBD_SHIFT_hnr:
-  \<open>(uncurry0 (return 2), uncurry0 (RETURN LBD_SHIFT) ) \<in> unit_assn\<^sup>k \<rightarrow>\<^sub>a uint64_nat_assn\<close>
-  by sepref_to_hoare (sep_auto simp: LBD_SHIFT_def uint64_nat_rel_def br_def)
-
-lemma MAX_LENGTH_SHORT_CLAUSE_hnr[sepref_fr_rules]:
-  \<open>(uncurry0 (return 4), uncurry0 (RETURN MAX_LENGTH_SHORT_CLAUSE)) \<in> unit_assn\<^sup>k \<rightarrow>\<^sub>a uint64_nat_assn\<close>
-  by sepref_to_hoare (sep_auto simp: uint64_nat_rel_def br_def)
-
-definition four_uint32 where \<open>four_uint32 = (4 :: uint32)\<close>
-
-lemma four_uint32_hnr:
-  \<open>(uncurry0 (return 4), uncurry0 (RETURN (four_uint32 :: uint32)) ) \<in> unit_assn\<^sup>k \<rightarrow>\<^sub>a uint32_assn\<close>
-  by sepref_to_hoare (sep_auto simp: uint32_nat_rel_def br_def four_uint32_def)
-
-lemma [sepref_fr_rules]:
-  \<open>(uncurry0 (return 5), uncurry0 (RETURN POS_SHIFT)) \<in> unit_assn\<^sup>k \<rightarrow>\<^sub>a nat_assn\<close>
-  by sepref_to_hoare (sep_auto simp: SHIFTS_def)
-
-lemma [sepref_fr_rules]:
-  \<open>(return o id, RETURN o xarena_lit) \<in> [is_Lit]\<^sub>a arena_el_assn\<^sup>k \<rightarrow> unat_lit_assn\<close>
-  by sepref_to_hoare (sep_auto simp: SIZE_SHIFT_def uint32_nat_rel_def unat_lit_rel_def
-    arena_el_rel_def br_def hr_comp_def split: arena_el.splits)
-
-sepref_definition isa_arena_length_code
-  is \<open>uncurry isa_arena_length\<close>
-  :: \<open>(arl_assn uint32_assn)\<^sup>k *\<^sub>a nat_assn\<^sup>k \<rightarrow>\<^sub>a uint64_assn\<close>
-  supply arena_el_assn_alt_def[symmetric, simp] sum_uint64_assn[sepref_fr_rules]
-  unfolding isa_arena_length_def
+sepref_register marked_as_used
+sepref_definition marked_as_used_impl 
+  is "uncurry (RETURN oo marked_as_used)" 
+    :: "[uncurry marked_as_used_pre]\<^sub>a arena_fast_assn\<^sup>k *\<^sub>a sint64_nat_assn\<^sup>k \<rightarrow> bool1_assn"
+  supply [intro] = arena_marked_as_used_implI
+  supply [simp] = max_snat_def
+  unfolding marked_as_used_def STATUS_SHIFT_def
+  apply (annot_snat_const "TYPE(64)")
   by sepref
+lemmas [sepref_fr_rules] = marked_as_used_impl.refine
 
-lemma isa_arena_length_code_refine[sepref_fr_rules]:
-  \<open>(uncurry isa_arena_length_code, uncurry (RETURN \<circ>\<circ> arena_length))
-  \<in> [uncurry arena_is_valid_clause_idx]\<^sub>a
-    arena_assn\<^sup>k *\<^sub>a nat_assn\<^sup>k \<rightarrow> uint64_nat_assn\<close>
-  using isa_arena_length_code.refine[FCOMP isa_arena_length_arena_length[unfolded convert_fref]]
-  unfolding hr_comp_assoc[symmetric] uncurry_def list_rel_compp
-  by (simp add: arl_assn_comp)
-
-sepref_definition isa_arena_length_fast_code
-  is \<open>uncurry isa_arena_length\<close>
-  :: \<open>(arl64_assn uint32_assn)\<^sup>k *\<^sub>a uint64_nat_assn\<^sup>k \<rightarrow>\<^sub>a uint64_assn\<close>
-  supply arena_el_assn_alt_def[symmetric, simp] sum_uint64_assn[sepref_fr_rules]
-    minus_uint64_nat_assn[sepref_fr_rules]
-  unfolding isa_arena_length_def SIZE_SHIFT_def fast_minus_def one_uint64_nat_def[symmetric]
+sepref_register MAX_LENGTH_SHORT_CLAUSE
+sepref_definition MAX_LENGTH_SHORT_CLAUSE_impl is "uncurry0 (RETURN MAX_LENGTH_SHORT_CLAUSE)" :: "unit_assn\<^sup>k \<rightarrow>\<^sub>a sint64_nat_assn"
+  unfolding MAX_LENGTH_SHORT_CLAUSE_def
+  apply (annot_snat_const "TYPE(64)")
+  supply [simp] = max_snat_def
   by sepref
+lemmas [sepref_fr_rules] = MAX_LENGTH_SHORT_CLAUSE_impl.refine
+    
 
-lemma isa_arena_length_fast_code_refine[sepref_fr_rules]:
-  \<open>(uncurry isa_arena_length_fast_code, uncurry (RETURN \<circ>\<circ> arena_length))
-  \<in> [uncurry arena_is_valid_clause_idx]\<^sub>a
-    arena_fast_assn\<^sup>k *\<^sub>a uint64_nat_assn\<^sup>k \<rightarrow> uint64_nat_assn\<close>
-  using isa_arena_length_fast_code.refine[FCOMP isa_arena_length_arena_length[unfolded convert_fref]]
-  unfolding hr_comp_assoc[symmetric] uncurry_def list_rel_compp
-  by (simp add: arl64_assn_comp)
-
-sepref_definition isa_arena_length_fast_code2
-  is \<open>uncurry isa_arena_length\<close>
-  :: \<open>(arl_assn uint32_assn)\<^sup>k *\<^sub>a uint64_nat_assn\<^sup>k \<rightarrow>\<^sub>a uint64_assn\<close>
-  supply arena_el_assn_alt_def[symmetric, simp] sum_uint64_assn[sepref_fr_rules]
-    minus_uint64_nat_assn[sepref_fr_rules]
-  unfolding isa_arena_length_def SIZE_SHIFT_def fast_minus_def one_uint64_nat_def[symmetric]
-  by sepref
-
-lemma isa_arena_length_fast_code2_refine[sepref_fr_rules]:
-  \<open>(uncurry isa_arena_length_fast_code2, uncurry (RETURN \<circ>\<circ> arena_length))
-  \<in> [uncurry arena_is_valid_clause_idx]\<^sub>a
-    arena_assn\<^sup>k *\<^sub>a uint64_nat_assn\<^sup>k \<rightarrow> uint64_nat_assn\<close>
-  using isa_arena_length_fast_code2.refine[FCOMP isa_arena_length_arena_length[unfolded convert_fref]]
-  unfolding hr_comp_assoc[symmetric] uncurry_def list_rel_compp
-  by (simp add: arl_assn_comp)
-
-sepref_definition isa_arena_lit_code
-  is \<open>uncurry isa_arena_lit\<close>
-  :: \<open>(arl_assn uint32_assn)\<^sup>k *\<^sub>a nat_assn\<^sup>k \<rightarrow>\<^sub>a uint32_assn\<close>
-  supply arena_el_assn_alt_def[symmetric, simp] sum_uint64_assn[sepref_fr_rules]
-  unfolding isa_arena_lit_def
-  by sepref
-
-lemma isa_arena_lit_code_refine[sepref_fr_rules]:
-  \<open>(uncurry isa_arena_lit_code, uncurry (RETURN \<circ>\<circ> arena_lit))
-  \<in> [uncurry arena_lit_pre]\<^sub>a
-    arena_assn\<^sup>k *\<^sub>a nat_assn\<^sup>k \<rightarrow> unat_lit_assn\<close>
-  using isa_arena_lit_code.refine[FCOMP isa_arena_lit_arena_lit[unfolded convert_fref]]
-  unfolding hr_comp_assoc[symmetric] uncurry_def list_rel_compp
-  by (simp add: arl_assn_comp)
-
-sepref_definition (in-) isa_arena_lit_fast_code
-  is \<open>uncurry isa_arena_lit\<close>
-  :: \<open>(arl64_assn uint32_assn)\<^sup>k *\<^sub>a uint64_nat_assn\<^sup>k \<rightarrow>\<^sub>a uint32_assn\<close>
-  supply arena_el_assn_alt_def[symmetric, simp] sum_uint64_assn[sepref_fr_rules]
-  unfolding isa_arena_lit_def
-  by sepref
-
-declare isa_arena_lit_fast_code.refine
-
-lemma isa_arena_lit_fast_code_refine[sepref_fr_rules]:
-  \<open>(uncurry isa_arena_lit_fast_code, uncurry (RETURN \<circ>\<circ> arena_lit))
-  \<in> [uncurry arena_lit_pre]\<^sub>a
-    arena_fast_assn\<^sup>k *\<^sub>a uint64_nat_assn\<^sup>k \<rightarrow> unat_lit_assn\<close>
-  using isa_arena_lit_fast_code.refine[FCOMP isa_arena_lit_arena_lit[unfolded convert_fref]]
-  unfolding hr_comp_assoc[symmetric] uncurry_def list_rel_compp
-  by (simp add: arl64_assn_comp)
-
-
-sepref_definition (in-) isa_arena_lit_fast_code2
-  is \<open>uncurry isa_arena_lit\<close>
-  :: \<open>(arl_assn uint32_assn)\<^sup>k *\<^sub>a uint64_nat_assn\<^sup>k \<rightarrow>\<^sub>a uint32_assn\<close>
-  supply arena_el_assn_alt_def[symmetric, simp] sum_uint64_assn[sepref_fr_rules]
-  unfolding isa_arena_lit_def
-  by sepref
-
-declare isa_arena_lit_fast_code2.refine
-
-lemma isa_arena_lit_fast_code2_refine[sepref_fr_rules]:
-  \<open>(uncurry isa_arena_lit_fast_code2, uncurry (RETURN \<circ>\<circ> arena_lit))
-  \<in> [uncurry arena_lit_pre]\<^sub>a
-    arena_assn\<^sup>k *\<^sub>a uint64_nat_assn\<^sup>k \<rightarrow> unat_lit_assn\<close>
-  using isa_arena_lit_fast_code2.refine[FCOMP isa_arena_lit_arena_lit[unfolded convert_fref]]
-  unfolding hr_comp_assoc[symmetric] uncurry_def list_rel_compp
-  by (simp add: arl_assn_comp)
-
-sepref_definition arena_status_code
-  is \<open>uncurry isa_arena_status\<close>
-  :: \<open>(arl_assn uint32_assn)\<^sup>k *\<^sub>a nat_assn\<^sup>k \<rightarrow>\<^sub>a uint32_assn\<close>
-  supply arena_el_assn_alt_def[symmetric, simp] sum_uint64_assn[sepref_fr_rules]
-  unfolding isa_arena_status_def
-  by sepref
-
-lemma isa_arena_status_refine[sepref_fr_rules]:
-  \<open>(uncurry arena_status_code, uncurry (RETURN \<circ>\<circ> arena_status))
-  \<in> [uncurry arena_is_valid_clause_vdom]\<^sub>a
-    arena_assn\<^sup>k *\<^sub>a nat_assn\<^sup>k \<rightarrow> status_assn\<close>
-  using arena_status_code.refine[FCOMP isa_arena_status_arena_status[unfolded convert_fref]]
-  unfolding hr_comp_assoc[symmetric] uncurry_def list_rel_compp status_assn_alt_def
-  by (simp add: arl_assn_comp)
-
-
-sepref_definition swap_lits_code
-  is \<open>Sepref_Misc.uncurry3 isa_arena_swap\<close>
-  :: \<open>nat_assn\<^sup>k *\<^sub>a nat_assn\<^sup>k *\<^sub>a nat_assn\<^sup>k *\<^sub>a (arl_assn uint32_assn)\<^sup>d  \<rightarrow>\<^sub>a arl_assn uint32_assn\<close>
-  unfolding isa_arena_swap_def WB_More_Refinement_List.swap_def IICF_List.swap_def[symmetric]
-  by sepref
-
-lemma swap_lits_refine[sepref_fr_rules]:
-  \<open>(uncurry3 swap_lits_code, uncurry3 (RETURN oooo swap_lits))
-  \<in> [uncurry3 swap_lits_pre]\<^sub>a nat_assn\<^sup>k *\<^sub>a nat_assn\<^sup>k *\<^sub>a nat_assn\<^sup>k *\<^sub>a arena_assn\<^sup>d \<rightarrow> arena_assn\<close>
-  using swap_lits_code.refine[FCOMP isa_arena_swap[unfolded convert_fref]]
-  unfolding hr_comp_assoc[symmetric] list_rel_compp status_assn_alt_def uncurry_def
-  by (auto simp add: arl_assn_comp)
-
-sepref_definition isa_update_lbd_code
-  is \<open>uncurry2 isa_update_lbd\<close>
-  :: \<open>nat_assn\<^sup>k *\<^sub>a uint32_assn\<^sup>k *\<^sub>a (arl_assn uint32_assn)\<^sup>d  \<rightarrow>\<^sub>a arl_assn uint32_assn\<close>
-  unfolding isa_update_lbd_def
-  by sepref
-
-
-lemma update_lbd_hnr[sepref_fr_rules]:
-  \<open>(uncurry2 isa_update_lbd_code, uncurry2 (RETURN ooo update_lbd))
-  \<in> [update_lbd_pre]\<^sub>a nat_assn\<^sup>k *\<^sub>a uint32_nat_assn\<^sup>k *\<^sub>a arena_assn\<^sup>d \<rightarrow> arena_assn\<close>
-  using isa_update_lbd_code.refine[FCOMP isa_update_lbd[unfolded convert_fref]]
-  unfolding hr_comp_assoc[symmetric] list_rel_compp status_assn_alt_def uncurry_def
-  by (auto simp add: arl_assn_comp update_lbd_pre_def)
-
-
-sepref_definition (in -)isa_update_lbd_fast_code
-  is \<open>uncurry2 isa_update_lbd\<close>
-  :: \<open>uint64_nat_assn\<^sup>k *\<^sub>a uint32_assn\<^sup>k *\<^sub>a (arl64_assn uint32_assn)\<^sup>d  \<rightarrow>\<^sub>a arl64_assn uint32_assn\<close>
-  supply LBD_SHIFT_hnr[sepref_fr_rules]
-  unfolding isa_update_lbd_def
-  by sepref
-
-lemma update_lbd_fast_hnr[sepref_fr_rules]:
-  \<open>(uncurry2 isa_update_lbd_fast_code, uncurry2 (RETURN ooo update_lbd))
-  \<in> [update_lbd_pre]\<^sub>a uint64_nat_assn\<^sup>k *\<^sub>a uint32_nat_assn\<^sup>k *\<^sub>a arena_fast_assn\<^sup>d \<rightarrow> arena_fast_assn\<close>
-  using isa_update_lbd_fast_code.refine[FCOMP isa_update_lbd[unfolded convert_fref]]
-  unfolding hr_comp_assoc[symmetric] list_rel_compp status_assn_alt_def uncurry_def
-  by (auto simp add: arl64_assn_comp update_lbd_pre_def)
-
-sepref_definition (in -)isa_update_lbd_fast_code2
-  is \<open>uncurry2 isa_update_lbd\<close>
-  :: \<open>uint64_nat_assn\<^sup>k *\<^sub>a uint32_assn\<^sup>k *\<^sub>a (arl_assn uint32_assn)\<^sup>d  \<rightarrow>\<^sub>a arl_assn uint32_assn\<close>
-  supply LBD_SHIFT_hnr[sepref_fr_rules]
-  unfolding isa_update_lbd_def
-  by sepref
-
-lemma update_lbd_fast_hnr2[sepref_fr_rules]:
-  \<open>(uncurry2 isa_update_lbd_fast_code2, uncurry2 (RETURN ooo update_lbd))
-  \<in> [update_lbd_pre]\<^sub>a uint64_nat_assn\<^sup>k *\<^sub>a uint32_nat_assn\<^sup>k *\<^sub>a arena_assn\<^sup>d \<rightarrow> arena_assn\<close>
-  using isa_update_lbd_fast_code2.refine[FCOMP isa_update_lbd[unfolded convert_fref]]
-  unfolding hr_comp_assoc[symmetric] list_rel_compp status_assn_alt_def uncurry_def
-  by (auto simp add: arl_assn_comp update_lbd_pre_def)
-
-sepref_definition isa_get_clause_LBD_code
-  is \<open>uncurry isa_get_clause_LBD\<close>
-  :: \<open>(arl_assn uint32_assn)\<^sup>k *\<^sub>a nat_assn\<^sup>k \<rightarrow>\<^sub>a uint32_assn\<close>
-  unfolding isa_get_clause_LBD_def fast_minus_def[symmetric]
-  by sepref
-
-lemma isa_get_clause_LBD_code[sepref_fr_rules]:
-  \<open>(uncurry isa_get_clause_LBD_code, uncurry (RETURN \<circ>\<circ> get_clause_LBD))
-     \<in> [uncurry get_clause_LBD_pre]\<^sub>a arena_assn\<^sup>k *\<^sub>a nat_assn\<^sup>k \<rightarrow> uint32_nat_assn\<close>
-  using isa_get_clause_LBD_code.refine[FCOMP isa_get_clause_LBD_get_clause_LBD[unfolded convert_fref]]
-  unfolding hr_comp_assoc[symmetric] list_rel_compp status_assn_alt_def uncurry_def
-  by (auto simp add: arl_assn_comp update_lbd_pre_def)
-
-sepref_definition isa_get_saved_pos_fast_code
-  is \<open>uncurry isa_get_saved_pos\<close>
-  :: \<open>(arl64_assn uint32_assn)\<^sup>k *\<^sub>a uint64_nat_assn\<^sup>k \<rightarrow>\<^sub>a uint64_assn\<close>
-  supply sum_uint64_assn[sepref_fr_rules] POS_SHIFT_uint64_hnr[sepref_fr_rules]
-  unfolding isa_get_saved_pos_def
-  by sepref
-
-lemma get_saved_pos_fast_code[sepref_fr_rules]:
-  \<open>(uncurry isa_get_saved_pos_fast_code, uncurry (RETURN \<circ>\<circ> arena_pos))
-     \<in> [uncurry get_saved_pos_pre]\<^sub>a arena_fast_assn\<^sup>k *\<^sub>a uint64_nat_assn\<^sup>k \<rightarrow> uint64_nat_assn\<close>
-  using isa_get_saved_pos_fast_code.refine[FCOMP isa_get_saved_pos_get_saved_pos[unfolded convert_fref]]
-  unfolding hr_comp_assoc[symmetric] list_rel_compp status_assn_alt_def uncurry_def
-  by (auto simp add: arl64_assn_comp update_lbd_pre_def)
-
-sepref_definition isa_get_saved_pos_code
-  is \<open>uncurry isa_get_saved_pos\<close>
-  :: \<open>(arl_assn uint32_assn)\<^sup>k *\<^sub>a nat_assn\<^sup>k \<rightarrow>\<^sub>a uint64_assn\<close>
-  supply sum_uint64_assn[sepref_fr_rules]
-  unfolding isa_get_saved_pos_def POS_SHIFT_def
-  by sepref
-
-lemma get_saved_pos_code[sepref_fr_rules]:
-  \<open>(uncurry isa_get_saved_pos_code, uncurry (RETURN \<circ>\<circ> arena_pos))
-     \<in> [uncurry get_saved_pos_pre]\<^sub>a arena_assn\<^sup>k *\<^sub>a nat_assn\<^sup>k \<rightarrow> uint64_nat_assn\<close>
-  using isa_get_saved_pos_code.refine[FCOMP isa_get_saved_pos_get_saved_pos[unfolded convert_fref]]
-  unfolding hr_comp_assoc[symmetric] list_rel_compp status_assn_alt_def uncurry_def
-  by (auto simp add: arl_assn_comp update_lbd_pre_def)
-
-sepref_definition isa_get_saved_pos_code'
-  is \<open>uncurry isa_get_saved_pos'\<close>
-  :: \<open>(arl_assn uint32_assn)\<^sup>k *\<^sub>a nat_assn\<^sup>k \<rightarrow>\<^sub>a nat_assn\<close>
-  supply sum_uint64_assn[sepref_fr_rules]
-  unfolding isa_get_saved_pos_def isa_get_saved_pos'_def
-  by sepref
-(* TODO check if we use this version anywhere *)
-lemma get_saved_pos_code':
-\<open>(uncurry isa_get_saved_pos_code', uncurry (RETURN \<circ>\<circ> arena_pos))
-     \<in> [uncurry get_saved_pos_pre]\<^sub>a arena_assn\<^sup>k *\<^sub>a nat_assn\<^sup>k \<rightarrow> nat_assn\<close>
-  using isa_get_saved_pos_code'.refine[FCOMP isa_get_saved_pos_get_saved_pos'[unfolded convert_fref]]
-  unfolding hr_comp_assoc[symmetric] list_rel_compp status_assn_alt_def uncurry_def
-  by (auto simp add: arl_assn_comp update_lbd_pre_def)
-
-sepref_definition isa_get_saved_pos_fast_code2
-  is \<open>uncurry isa_get_saved_pos\<close>
-  :: \<open>(arl_assn uint32_assn)\<^sup>k *\<^sub>a uint64_nat_assn\<^sup>k \<rightarrow>\<^sub>a uint64_assn\<close>
-  supply sum_uint64_assn[sepref_fr_rules] POS_SHIFT_uint64_hnr[sepref_fr_rules]
-  unfolding isa_get_saved_pos_def
-  by sepref
-
-lemma get_saved_pos_code2[sepref_fr_rules]:
-  \<open>(uncurry isa_get_saved_pos_fast_code2, uncurry (RETURN \<circ>\<circ> arena_pos))
-     \<in> [uncurry get_saved_pos_pre]\<^sub>a arena_assn\<^sup>k *\<^sub>a uint64_nat_assn\<^sup>k \<rightarrow> uint64_nat_assn\<close>
-  using isa_get_saved_pos_fast_code2.refine[FCOMP isa_get_saved_pos_get_saved_pos[unfolded convert_fref]]
-  unfolding hr_comp_assoc[symmetric] list_rel_compp status_assn_alt_def uncurry_def
-  by (auto simp add: arl_assn_comp update_lbd_pre_def)
-
-sepref_definition isa_update_pos_code
-  is \<open>uncurry2 isa_update_pos\<close>
-  :: \<open>nat_assn\<^sup>k *\<^sub>a nat_assn\<^sup>k *\<^sub>a (arl_assn uint32_assn)\<^sup>d  \<rightarrow>\<^sub>a arl_assn uint32_assn\<close>
-  supply minus_uint32_assn[sepref_fr_rules]
-  unfolding isa_update_pos_def
-  by sepref
-
-lemma isa_update_pos_code_hnr[sepref_fr_rules]:
-  \<open>(uncurry2 isa_update_pos_code, uncurry2 (RETURN ooo arena_update_pos))
-  \<in> [isa_update_pos_pre]\<^sub>a nat_assn\<^sup>k *\<^sub>a nat_assn\<^sup>k *\<^sub>a arena_assn\<^sup>d \<rightarrow> arena_assn\<close>
-  using isa_update_pos_code.refine[FCOMP isa_update_pos[unfolded convert_fref]]
-  unfolding hr_comp_assoc[symmetric] list_rel_compp status_assn_alt_def uncurry_def
-  by (auto simp add: arl_assn_comp isa_update_pos_pre_def)
-
-sepref_definition mark_garbage_code
-  is \<open>uncurry mark_garbage\<close>
-  :: \<open>(arl_assn uint32_assn)\<^sup>d *\<^sub>a nat_assn\<^sup>k \<rightarrow>\<^sub>a arl_assn uint32_assn\<close>
-  unfolding mark_garbage_def fast_minus_def[symmetric]
-  by sepref
-
-lemma mark_garbage_hnr[sepref_fr_rules]:
-  \<open>(uncurry mark_garbage_code, uncurry (RETURN oo extra_information_mark_to_delete))
-  \<in> [mark_garbage_pre]\<^sub>a  arena_assn\<^sup>d *\<^sub>a nat_assn\<^sup>k \<rightarrow> arena_assn\<close>
-  using mark_garbage_code.refine[FCOMP isa_mark_garbage[unfolded convert_fref]]
-  unfolding hr_comp_assoc[symmetric] list_rel_compp status_assn_alt_def uncurry_def
-  by (auto simp add: arl_assn_comp update_lbd_pre_def)
-
-sepref_definition isa_arena_act_code
-  is \<open>uncurry isa_arena_act\<close>
-  :: \<open>(arl_assn uint32_assn)\<^sup>k *\<^sub>a nat_assn\<^sup>k \<rightarrow>\<^sub>a uint32_assn\<close>
-  unfolding isa_arena_act_def ACTIVITY_SHIFT_def fast_minus_def[symmetric]
-  by sepref
-
-lemma isa_arena_act_code[sepref_fr_rules]:
-  \<open>(uncurry isa_arena_act_code, uncurry (RETURN \<circ>\<circ> arena_act))
-     \<in> [uncurry arena_act_pre]\<^sub>a arena_assn\<^sup>k *\<^sub>a nat_assn\<^sup>k \<rightarrow> uint32_nat_assn\<close>
-  using isa_arena_act_code.refine[FCOMP isa_arena_act_arena_act[unfolded convert_fref]]
-  unfolding hr_comp_assoc[symmetric] list_rel_compp status_assn_alt_def uncurry_def
-  by (auto simp add: arl_assn_comp update_lbd_pre_def)
-
-sepref_definition isa_arena_incr_act_code
-  is \<open>uncurry isa_arena_incr_act\<close>
-  :: \<open>(arl_assn uint32_assn)\<^sup>d *\<^sub>a nat_assn\<^sup>k \<rightarrow>\<^sub>a (arl_assn uint32_assn)\<close>
-  unfolding isa_arena_incr_act_def ACTIVITY_SHIFT_def fast_minus_def
-  by sepref
-
-lemma isa_arena_incr_act_code[sepref_fr_rules]:
-  \<open>(uncurry isa_arena_incr_act_code, uncurry (RETURN \<circ>\<circ> arena_incr_act))
-     \<in> [uncurry arena_act_pre]\<^sub>a arena_assn\<^sup>d *\<^sub>a nat_assn\<^sup>k \<rightarrow> arena_assn\<close>
-  using isa_arena_incr_act_code.refine[FCOMP isa_arena_incr_act_arena_incr_act[unfolded convert_fref]]
-  unfolding hr_comp_assoc[symmetric] list_rel_compp status_assn_alt_def uncurry_def
-  by (auto simp add: arl_assn_comp update_lbd_pre_def)
-
-sepref_definition isa_arena_decr_act_code
-  is \<open>uncurry isa_arena_decr_act\<close>
-  :: \<open>(arl_assn uint32_assn)\<^sup>d *\<^sub>a nat_assn\<^sup>k \<rightarrow>\<^sub>a (arl_assn uint32_assn)\<close>
-  unfolding isa_arena_decr_act_def ACTIVITY_SHIFT_def fast_minus_def
-  by sepref
-
-lemma isa_arena_decr_act_code[sepref_fr_rules]:
-  \<open>(uncurry isa_arena_decr_act_code, uncurry (RETURN \<circ>\<circ> arena_decr_act))
-     \<in> [uncurry arena_act_pre]\<^sub>a arena_assn\<^sup>d *\<^sub>a nat_assn\<^sup>k \<rightarrow> arena_assn\<close>
-  using isa_arena_decr_act_code.refine[FCOMP isa_arena_decr_act_arena_decr_act[unfolded convert_fref]]
-  unfolding hr_comp_assoc[symmetric] list_rel_compp status_assn_alt_def uncurry_def
-  by (auto simp add: arl_assn_comp update_lbd_pre_def)
-
-
-sepref_definition isa_arena_decr_act_fast_code
-  is \<open>uncurry isa_arena_decr_act\<close>
-  :: \<open>(arl64_assn uint32_assn)\<^sup>d *\<^sub>a uint64_nat_assn\<^sup>k \<rightarrow>\<^sub>a (arl64_assn uint32_assn)\<close>
-  unfolding isa_arena_decr_act_def
-  three_uint32_def[symmetric] ACTIVITY_SHIFT_hnr[sepref_fr_rules]
-  by sepref
-
-lemma isa_arena_decr_act_fast_code[sepref_fr_rules]:
-  \<open>(uncurry isa_arena_decr_act_fast_code, uncurry (RETURN \<circ>\<circ> arena_decr_act))
-     \<in> [uncurry arena_act_pre]\<^sub>a arena_fast_assn\<^sup>d *\<^sub>a uint64_nat_assn\<^sup>k \<rightarrow> arena_fast_assn\<close>
-  using isa_arena_decr_act_fast_code.refine[FCOMP isa_arena_decr_act_arena_decr_act[unfolded convert_fref]]
-  unfolding hr_comp_assoc[symmetric] list_rel_compp status_assn_alt_def uncurry_def
-  by (auto simp add: arl64_assn_comp update_lbd_pre_def)
-
-sepref_definition isa_mark_used_code
-  is \<open>uncurry isa_mark_used\<close>
-  :: \<open>(arl_assn uint32_assn)\<^sup>d *\<^sub>a nat_assn\<^sup>k \<rightarrow>\<^sub>a (arl_assn uint32_assn)\<close>
-  unfolding isa_mark_used_def ACTIVITY_SHIFT_def fast_minus_def[symmetric]
-  by sepref
-
-lemma isa_mark_used_code[sepref_fr_rules]:
-  \<open>(uncurry isa_mark_used_code, uncurry (RETURN \<circ>\<circ> mark_used))
-     \<in> [uncurry arena_act_pre]\<^sub>a arena_assn\<^sup>d *\<^sub>a nat_assn\<^sup>k \<rightarrow> arena_assn\<close>
-  using isa_mark_used_code.refine[FCOMP isa_mark_used_mark_used[unfolded convert_fref]]
-  unfolding hr_comp_assoc[symmetric] list_rel_compp status_assn_alt_def uncurry_def
-  by (auto simp add: arl_assn_comp update_lbd_pre_def)
-
-
-sepref_definition isa_mark_used_fast_code
-  is \<open>uncurry isa_mark_used\<close>
-  :: \<open>(arl_assn uint32_assn)\<^sup>d *\<^sub>a uint64_nat_assn\<^sup>k \<rightarrow>\<^sub>a (arl_assn uint32_assn)\<close>
-  supply four_uint32_hnr[sepref_fr_rules] STATUS_SHIFT_hnr[sepref_fr_rules]
-  unfolding isa_mark_used_def four_uint32_def[symmetric]
-  by sepref
-
-lemma isa_mark_used_fast_code[sepref_fr_rules]:
-  \<open>(uncurry isa_mark_used_fast_code, uncurry (RETURN \<circ>\<circ> mark_used))
-     \<in> [uncurry arena_act_pre]\<^sub>a arena_assn\<^sup>d *\<^sub>a uint64_nat_assn\<^sup>k \<rightarrow> arena_assn\<close>
-  using isa_mark_used_fast_code.refine[FCOMP isa_mark_used_mark_used[unfolded convert_fref]]
-  unfolding hr_comp_assoc[symmetric] list_rel_compp status_assn_alt_def uncurry_def
-  by (auto simp add: arl_assn_comp update_lbd_pre_def)
-
-sepref_definition isa_mark_unused_code
-  is \<open>uncurry isa_mark_unused\<close>
-  :: \<open>(arl_assn uint32_assn)\<^sup>d *\<^sub>a nat_assn\<^sup>k \<rightarrow>\<^sub>a (arl_assn uint32_assn)\<close>
-  unfolding isa_mark_unused_def ACTIVITY_SHIFT_def fast_minus_def[symmetric]
-  by sepref
-
-lemma isa_mark_unused_code[sepref_fr_rules]:
-  \<open>(uncurry isa_mark_unused_code, uncurry (RETURN \<circ>\<circ> mark_unused))
-     \<in> [uncurry arena_act_pre]\<^sub>a arena_assn\<^sup>d *\<^sub>a nat_assn\<^sup>k \<rightarrow> arena_assn\<close>
-  using isa_mark_unused_code.refine[FCOMP isa_mark_unused_mark_unused[unfolded convert_fref]]
-  unfolding hr_comp_assoc[symmetric] list_rel_compp status_assn_alt_def uncurry_def
-  by (auto simp add: arl_assn_comp update_lbd_pre_def)
-
-sepref_definition isa_mark_unused_fast_code
-  is \<open>uncurry isa_mark_unused\<close>
-  :: \<open>(arl_assn uint32_assn)\<^sup>d *\<^sub>a uint64_nat_assn\<^sup>k \<rightarrow>\<^sub>a (arl_assn uint32_assn)\<close>
-  supply STATUS_SHIFT_hnr[sepref_fr_rules]
-  unfolding isa_mark_unused_def ACTIVITY_SHIFT_def fast_minus_def[symmetric]
-  by sepref
-
-
-lemma isa_mark_unused_fast_code[sepref_fr_rules]:
-  \<open>(uncurry isa_mark_unused_fast_code, uncurry (RETURN \<circ>\<circ> mark_unused))
-     \<in> [uncurry arena_act_pre]\<^sub>a arena_assn\<^sup>d *\<^sub>a uint64_nat_assn\<^sup>k \<rightarrow> arena_assn\<close>
-  using isa_mark_unused_fast_code.refine[FCOMP isa_mark_unused_mark_unused[unfolded convert_fref]]
-  unfolding hr_comp_assoc[symmetric] list_rel_compp status_assn_alt_def uncurry_def
-  by (auto simp add: arl_assn_comp update_lbd_pre_def)
-
-sepref_definition isa_marked_as_used_code
-  is \<open>uncurry isa_marked_as_used\<close>
-  :: \<open>(arl_assn uint32_assn)\<^sup>k *\<^sub>a nat_assn\<^sup>k \<rightarrow>\<^sub>a bool_assn\<close>
-  supply op_eq_uint32[sepref_fr_rules]
-  unfolding isa_marked_as_used_def fast_minus_def[symmetric]
-  by sepref
-
-
-
-lemma isa_marked_as_used_code[sepref_fr_rules]:
-  \<open>(uncurry isa_marked_as_used_code, uncurry (RETURN \<circ>\<circ> marked_as_used))
-     \<in> [uncurry marked_as_used_pre]\<^sub>a arena_assn\<^sup>k *\<^sub>a nat_assn\<^sup>k \<rightarrow> bool_assn\<close>
-  using isa_marked_as_used_code.refine[FCOMP isa_marked_as_used_marked_as_used[unfolded convert_fref]]
-  unfolding hr_comp_assoc[symmetric] list_rel_compp status_assn_alt_def uncurry_def
-  by (auto simp add: arl_assn_comp update_lbd_pre_def)
-
-
-
-sepref_definition (in -) isa_arena_incr_act_fast_code
-  is \<open>uncurry isa_arena_incr_act\<close>
-  :: \<open>(arl64_assn uint32_assn)\<^sup>d *\<^sub>a uint64_nat_assn\<^sup>k \<rightarrow>\<^sub>a (arl64_assn uint32_assn)\<close>
-  supply ACTIVITY_SHIFT_hnr[sepref_fr_rules]
-  unfolding isa_arena_incr_act_def
-  by sepref
-
-lemma isa_arena_incr_act_fast_code[sepref_fr_rules]:
-  \<open>(uncurry isa_arena_incr_act_fast_code, uncurry (RETURN \<circ>\<circ> arena_incr_act))
-     \<in> [uncurry arena_act_pre]\<^sub>a arena_fast_assn\<^sup>d *\<^sub>a uint64_nat_assn\<^sup>k \<rightarrow> arena_fast_assn\<close>
-  using isa_arena_incr_act_fast_code.refine[FCOMP isa_arena_incr_act_arena_incr_act[unfolded convert_fref]]
-  unfolding hr_comp_assoc[symmetric] list_rel_compp status_assn_alt_def uncurry_def
-  by (auto simp add: arl64_assn_comp update_lbd_pre_def)
-
-sepref_definition arena_status_fast_code
-  is \<open>uncurry isa_arena_status\<close>
-  :: \<open>(arl64_assn uint32_assn)\<^sup>k *\<^sub>a uint64_nat_assn\<^sup>k \<rightarrow>\<^sub>a uint32_assn\<close>
-  supply arena_el_assn_alt_def[symmetric, simp] sum_uint64_assn[sepref_fr_rules]
-    three_uint32_hnr[sepref_fr_rules] STATUS_SHIFT_hnr[sepref_fr_rules]
-  unfolding isa_arena_status_def three_uint32_def[symmetric]
-  by sepref
-
-lemma isa_arena_status_fast_hnr[sepref_fr_rules]:
-  \<open>(uncurry arena_status_fast_code, uncurry (RETURN \<circ>\<circ> arena_status))
-  \<in> [uncurry arena_is_valid_clause_vdom]\<^sub>a
-    arena_fast_assn\<^sup>k *\<^sub>a uint64_nat_assn\<^sup>k \<rightarrow> status_assn\<close>
-  using arena_status_fast_code.refine[FCOMP isa_arena_status_arena_status[unfolded convert_fref]]
-  unfolding hr_comp_assoc[symmetric] uncurry_def list_rel_compp status_assn_alt_def
-  by (simp add: arl64_assn_comp)
-
-context
-  notes [fcomp_norm_unfold] = arl64_assn_def[symmetric] arl64_assn_comp'
-  notes [intro!] = hfrefI hn_refineI[THEN hn_refine_preI]
-  notes [simp] = pure_def hn_ctxt_def invalid_assn_def
-begin
-
-definition arl64_get2 :: "'a::heap array_list64 \<Rightarrow> nat \<Rightarrow> 'a Heap" where
-  "arl64_get2 \<equiv> \<lambda>(a,n) i. Array.nth a i"
-thm arl64_get_hnr_aux
-lemma arl64_get2_hnr_aux: "(uncurry arl64_get2,uncurry (RETURN oo op_list_get)) \<in> [\<lambda>(l,i). i<length l]\<^sub>a (is_array_list64\<^sup>k *\<^sub>a nat_assn\<^sup>k) \<rightarrow> id_assn"
-    by sepref_to_hoare (sep_auto simp: arl64_get2_def is_array_list64_def)
-
-  sepref_decl_impl arl64_get2: arl64_get2_hnr_aux .
 end
 
-sepref_definition arena_status_fast_code2
-  is \<open>uncurry isa_arena_status\<close>
-  :: \<open>(arl64_assn uint32_assn)\<^sup>k *\<^sub>a nat_assn\<^sup>k \<rightarrow>\<^sub>a uint32_assn\<close>
-  supply arena_el_assn_alt_def[symmetric, simp] sum_uint64_assn[sepref_fr_rules]
-    three_uint32_hnr[sepref_fr_rules]
-  unfolding isa_arena_status_def STATUS_SHIFT_def fast_minus_def
-  by sepref
-
-lemma isa_arena_status_fast_hnr2[sepref_fr_rules]:
-  \<open>(uncurry arena_status_fast_code2, uncurry (RETURN \<circ>\<circ> arena_status))
-  \<in> [uncurry arena_is_valid_clause_vdom]\<^sub>a
-    arena_fast_assn\<^sup>k *\<^sub>a nat_assn\<^sup>k \<rightarrow> status_assn\<close>
-  using arena_status_fast_code2.refine[FCOMP isa_arena_status_arena_status[unfolded convert_fref]]
-  unfolding hr_comp_assoc[symmetric] uncurry_def list_rel_compp status_assn_alt_def
-  by (simp add: arl64_assn_comp)
-
-sepref_definition isa_update_pos_fast_code
-  is \<open>uncurry2 isa_update_pos\<close>
-  :: \<open>uint64_nat_assn\<^sup>k *\<^sub>a uint64_nat_assn\<^sup>k *\<^sub>a (arl64_assn uint32_assn)\<^sup>d  \<rightarrow>\<^sub>a arl64_assn uint32_assn\<close>
-  supply minus_uint32_assn[sepref_fr_rules] POS_SHIFT_uint64_hnr[sepref_fr_rules] minus_uint64_assn[sepref_fr_rules]
-  unfolding isa_update_pos_def  uint32_nat_assn_minus[sepref_fr_rules] two_uint64_nat_def[symmetric]
-  by sepref
-
-lemma isa_update_pos_code_fast_hnr[sepref_fr_rules]:
-  \<open>(uncurry2 isa_update_pos_fast_code, uncurry2 (RETURN ooo arena_update_pos))
-  \<in> [isa_update_pos_pre]\<^sub>a uint64_nat_assn\<^sup>k *\<^sub>a uint64_nat_assn\<^sup>k *\<^sub>a arena_fast_assn\<^sup>d \<rightarrow> arena_fast_assn\<close>
-  using isa_update_pos_fast_code.refine[FCOMP isa_update_pos[unfolded convert_fref]]
-  unfolding hr_comp_assoc[symmetric] list_rel_compp status_assn_alt_def uncurry_def
-  by (auto simp add: arl64_assn_comp isa_update_pos_pre_def)
-
-declare isa_update_pos_fast_code.refine[sepref_fr_rules]
-  arena_status_fast_code.refine[sepref_fr_rules]
-
-end
